src/TV/symexe_complete.v
@@ -1,0 +1,539 @@
+Add LoadPath "../ssa/ott".
+Add LoadPath "../ssa/monads".
+Add LoadPath "../ssa".
+Add LoadPath "../../../theory/metatheory".
+Require Import ssa.
+Require Import List.
+Require Export targetdata.
+Require Import monad.
+Require Import Arith.
+Require Import Metatheory.
+Require Import ssa_mem.
+Require Import genericvalues.
+Require Import ssa_dynamic.
+Require Import trace.
+Require Import symexe_def.
+
+Export SimpleSE.
+
+(* Symbolic execuction is complete:
+   Any concrete execution of a subblock satisfies its symbolic execution. *)
+
+Lemma genericvalue__implies__value2Sterm_denotes : forall TD lc0 gl0 Mem0 smap1 lc gl v gv,
+  uniq smap1 ->
+  smap_denotes_gvmap TD lc0 gl0 Mem0 smap1 lc gl ->
+  getOperandValue TD v lc gl = Some gv ->
+  sterm_denotes_genericvalue TD lc0 gl0 Mem0 (value2Sterm smap1 v) gv.
+Proof.
+  intros D lc0 gl0 Mem0 smap1 lc gl v gv Huniq Hdenotes J.
+  unfold getOperandValue in J.
+  unfold smap_denotes_gvmap in Hdenotes.
+  destruct Hdenotes as [J1 J2].
+  destruct v.
+    apply J2 in J.
+    destruct J as [st0 [J3 J4]].
+    rewrite id2Sterm_in with (st0:=st0); auto.
+
+    rewrite const2Sterm; auto.
+Qed.
+
+Lemma genericvalues__imply__value2Sterm_denote : forall l0 TD lc0 gl0 Mem0 smap1 lc gl gvs0,
+  uniq smap1 ->
+  (dom lc0 `union` dom gl0) [<=] dom smap1 ->
+  smap_denotes_gvmap TD lc0 gl0 Mem0 smap1 lc gl ->
+  values2GVs TD l0 lc gl = Some gvs0 ->
+  sterms_denote_genericvalues TD lc0 gl0 Mem0 
+    (List.map (value2Sterm smap1) l0) gvs0.
+Proof.
+  induction l0; intros; simpl in *.
+    inversion H2; subst; auto.
+
+    remember (getOperandValue TD a lc gl) as ogv.
+    destruct ogv; try solve [inversion H2].
+    remember (values2GVs TD l0 lc gl) as ogvs.
+    destruct ogvs; try solve [inversion H2].
+    inversion H2; subst.
+    apply sterms_cons_denote; eauto using genericvalue__implies__value2Sterm_denotes.
+Qed.
+
+Lemma se_cmd__denotes__op_cmd__case1 : forall lc gl i0 gv3 lc' gl' id' st' smap1 TD lc0 gl0 Mem0,
+  updateEnv lc gl i0 gv3 = (lc', gl') ->
+  i0 <> id' ->
+  binds id' st' smap1 ->
+  smap_denotes_gvmap TD lc0 gl0 Mem0 smap1 lc gl ->
+  exists gv',
+    sterm_denotes_genericvalue TD lc0 gl0 Mem0 st' gv' /\
+    lookupEnv id' lc' gl' = Some gv'.
+Proof.
+  intros lc gl i0 gv3 lc' gl' id' st' smap1 TD lc0 gl0 Mem0 H25 nEQ Hbinds Hsterm_denotes.
+  apply lookupEnv_updateEnv_neq with (id1:=id') in H25; auto.
+  rewrite <- H25. 
+  unfold smap_denotes_gvmap in Hsterm_denotes.
+  destruct Hsterm_denotes as [J1 J2].
+  apply J1 in Hbinds.
+  destruct Hbinds as [gv' [J3 J4]].
+  exists gv'. split; auto.
+Qed.
+
+Lemma se_cmd__denotes__op_cmd__case2 : forall lc gl i0 gv3 lc' gl' id' smap1 TD lc0 gl0 Mem0 gv' st0,
+  updateEnv lc gl i0 gv3 = (lc', gl') ->
+  smap_denotes_gvmap TD lc0 gl0 Mem0 smap1 lc gl ->
+  lookupEnv id' lc' gl' = Some gv' ->
+  id' <> i0 ->
+  exists st', binds id' st' (updateSmap smap1 i0 st0) /\ 
+              sterm_denotes_genericvalue TD lc0 gl0 Mem0 st' gv'.
+Proof.
+  intros lc gl i0 gv3 lc' gl' id' smap1 TD lc0 gl0 Mem0 gv' st0 H25 Hsterm_denotes HlookupEnv n.
+  apply lookupEnv_updateEnv_neq with (id1:=id') in H25; auto.
+  rewrite <- H25 in HlookupEnv.
+  destruct Hsterm_denotes as [J1 J2].
+  apply J2 in HlookupEnv; auto.
+  destruct HlookupEnv as [st' [J3 J4]].
+  exists st'. split; auto.
+    apply binds_updateSmap_neq; auto.
+Qed.
+
+Lemma op_cmd__satisfies__se_cmd : forall S TD Ps F B c cs call0 sbs tmn lc arg als ECs gl lc0 gl0 als0 Mem0 lc' als' gl' Mem1 Mem2 sstate1 tr tr1,
+  dbCmd (mkState S TD Ps ((mkEC F B ((subblock_intro (c::cs) call0)::sbs) tmn lc arg als)::ECs) gl Mem1)
+         (mkState S TD Ps ((mkEC F B ((subblock_intro cs call0)::sbs) tmn lc' arg als')::ECs) gl' Mem2)
+         tr -> 
+  uniq sstate1.(STerms) ->
+  (dom lc0 `union` dom gl0) [<=] dom (STerms sstate1) ->
+  sstate_denotes_state TD lc0 gl0 als0 Mem0 sstate1 lc gl als Mem1 tr1 ->
+  sstate_denotes_state TD lc0 gl0 als0 Mem0 (se_cmd sstate1 c) lc' gl' als' Mem2 (trace_app tr1 tr).
+Proof.
+  intros S TD Ps F B c cs call0 sbs tmn lc arg0 als ECs gl lc0 gl0 als0 Mem0 lc' als' gl' Mem1 Mem2 sstate1 tr tr1 HdsInsn Huniq Hsub Hdenotes.
+  (cmd_cases (destruct c;
+              inversion HdsInsn; subst;
+              destruct Hdenotes as [Hsterm_denotes [Hsmem_denotes [Hsframe_denotes Hseffects_denote]]];
+              rewrite trace_app_nil__eq__trace) Case).
+  Case "insn_bop".
+    split; auto.
+      split.
+        intros id' st' Hbinds.
+        simpl in Hbinds. simpl_env in Hbinds.
+        analyze_binds Hbinds.
+        apply updateSmap_inversion in Hbinds; auto.
+        destruct Hbinds as [[nEQ Hbinds] | [EQ1 EQ2]]; subst.
+          eapply se_cmd__denotes__op_cmd__case1; eauto.
+
+          apply lookupEnv_updateEnv_eq in H25; auto.
+          rewrite H25.
+          apply BOP_inversion in H24.
+          destruct H24 as [gv1 [gv2 [J1 [J2 J3]]]].
+          exists gv3. split; auto.
+          apply sterm_bop_denotes with (gv1:=gv1)(gv2:=gv2); eauto using genericvalue__implies__value2Sterm_denotes.
+
+        intros id' gv' HlookupEnv.
+        simpl. 
+        destruct (id'==i0); subst.
+          exists (sterm_bop b s (value2Sterm (STerms sstate1) v) (value2Sterm (STerms sstate1) v0)).
+          split. 
+            apply binds_updateSmap_eq; auto.
+
+            apply lookupEnv_updateEnv_eq in H25; auto.
+            rewrite H25 in HlookupEnv.
+            inversion HlookupEnv; subst.
+            apply BOP_inversion in H24.
+            destruct H24 as [gv1 [gv2 [J1 [J2 J3]]]].
+            apply sterm_bop_denotes with (gv1:=gv1)(gv2:=gv2); eauto using genericvalue__implies__value2Sterm_denotes.
+
+          eapply se_cmd__denotes__op_cmd__case2; eauto.
+
+  Case "insn_extractvalue".
+    split; auto.
+      split.
+        intros id' st' Hbinds.
+        simpl in Hbinds. simpl_env in Hbinds.
+        analyze_binds Hbinds.
+        apply updateSmap_inversion in Hbinds; auto.
+        destruct Hbinds as [[nEQ Hbinds] | [EQ1 EQ2]]; subst.
+          eapply se_cmd__denotes__op_cmd__case1; eauto.
+
+          apply lookupEnv_updateEnv_eq in H25; auto.
+          rewrite H25.
+          exists gv'. split; auto.
+          apply sterm_extractvalue_denotes with (gv1:=gv); eauto using genericvalue__implies__value2Sterm_denotes.
+
+        intros id' gv'0 HlookupEnv.
+        simpl. 
+        destruct (id'==i0); subst.
+          exists (sterm_extractvalue t (value2Sterm (STerms sstate1) v) l0).
+          split. 
+            apply binds_updateSmap_eq; auto.
+
+            apply lookupEnv_updateEnv_eq in H25; auto.
+            rewrite H25 in HlookupEnv.
+            inversion HlookupEnv; subst.
+            apply sterm_extractvalue_denotes with (gv1:=gv); eauto using genericvalue__implies__value2Sterm_denotes.
+
+          eapply se_cmd__denotes__op_cmd__case2; eauto.
+
+  Case "insn_insertvalue".
+    split; auto.
+      split.
+        intros id' st' Hbinds.
+        simpl in Hbinds. simpl_env in Hbinds.
+        analyze_binds Hbinds.
+        apply updateSmap_inversion in Hbinds; auto.
+        destruct Hbinds as [[nEQ Hbinds] | [EQ1 EQ2]]; subst.
+          eapply se_cmd__denotes__op_cmd__case1; eauto.
+
+          apply lookupEnv_updateEnv_eq in H28; auto.
+          rewrite H28.
+          exists gv''. split; auto.
+          eapply sterm_insertvalue_denotes; eauto using genericvalue__implies__value2Sterm_denotes.
+
+        intros id' gv'0 HlookupEnv.
+        simpl. 
+        destruct (id'==i0); subst.
+          exists (sterm_insertvalue t (value2Sterm(STerms sstate1) v) t0 (value2Sterm (STerms sstate1) v0) l0).
+          split. 
+            apply binds_updateSmap_eq; auto.
+
+            apply lookupEnv_updateEnv_eq in H28; auto.
+            rewrite H28 in HlookupEnv.
+            inversion HlookupEnv; subst.
+            eapply sterm_insertvalue_denotes; eauto using genericvalue__implies__value2Sterm_denotes.
+
+          eapply se_cmd__denotes__op_cmd__case2; eauto.
+
+  Case "insn_malloc".
+    split; simpl; eauto.
+      split.
+        intros id' st' Hbinds.
+        simpl in Hbinds. simpl_env in Hbinds.
+        analyze_binds Hbinds.
+        apply updateSmap_inversion in Hbinds; auto.
+        destruct Hbinds as [[nEQ Hbinds] | [EQ1 EQ2]]; subst.
+          eapply se_cmd__denotes__op_cmd__case1; eauto.
+
+          apply lookupEnv_updateEnv_eq in H25; auto.
+          rewrite H25.
+          exists (ptr2GV TD (mb, 0)).
+          split; auto.
+            eapply sterm_malloc_denotes; eauto.
+
+        intros id' gv'0 HlookupEnv.
+        simpl.
+        destruct (id'==i0); subst.
+          exists (sterm_malloc (SMem sstate1) t s a).
+          split. 
+            apply binds_updateSmap_eq; auto.
+
+            apply lookupEnv_updateEnv_eq in H25; auto.
+            rewrite H25 in HlookupEnv.
+            inversion HlookupEnv; subst.
+            eapply sterm_malloc_denotes; eauto.
+
+          eapply se_cmd__denotes__op_cmd__case2; eauto.
+
+  Case "insn_free".
+    split; simpl.
+      destruct Hsterm_denotes as [J1 J2].
+      split; auto.
+    split; auto.     
+      apply getOperandPtr_inversion in H22.
+      destruct H22 as [gv [J1 J2]].
+      apply smem_free_denotes with (Mem1:=Mem1)(gv0:=gv)(mptr0:=mptr); auto.
+        eapply genericvalue__implies__value2Sterm_denotes; eauto.
+    
+  Case "insn_alloca".
+    split; simpl; eauto.
+      split.
+        intros id' st' Hbinds.
+        simpl in Hbinds. simpl_env in Hbinds.
+        analyze_binds Hbinds.
+        apply updateSmap_inversion in Hbinds; auto.
+        destruct Hbinds as [[nEQ Hbinds] | [EQ1 EQ2]]; subst.
+          eapply se_cmd__denotes__op_cmd__case1; eauto.
+
+          apply lookupEnv_updateEnv_eq in H25; auto.
+          rewrite H25.
+          exists (ptr2GV TD (mb, 0)).
+          split; auto.
+          eapply sterm_alloca_denotes; eauto.
+
+        intros id' gv'0 HlookupEnv.
+        simpl.
+        destruct (id'==i0); subst.
+          exists (sterm_alloca (SMem sstate1) t s a).
+          split. 
+            apply binds_updateSmap_eq; auto.
+
+            apply lookupEnv_updateEnv_eq in H25; auto.
+            rewrite H25 in HlookupEnv.
+            inversion HlookupEnv; subst.
+            eapply sterm_alloca_denotes; eauto.
+
+          eapply se_cmd__denotes__op_cmd__case2; eauto.
+
+  Case "insn_load".
+    split; simpl; eauto.
+      apply getOperandPtr_inversion in H22.
+      destruct H22 as [gv2 [J1 J2]].
+      split.
+        intros id' st' Hbinds.
+        simpl in Hbinds. simpl_env in Hbinds.
+        analyze_binds Hbinds.
+        apply updateSmap_inversion in Hbinds; auto.
+        destruct Hbinds as [[nEQ Hbinds] | [EQ1 EQ2]]; subst.
+          eapply se_cmd__denotes__op_cmd__case1; eauto.
+
+          apply lookupEnv_updateEnv_eq in H24; auto.
+          rewrite H24.
+          exists gv.
+          split; auto.
+          apply sterm_load_denotes with (Mem1:=Mem2)(gv0:=gv2)(mp0:=mp); eauto.
+            eapply genericvalue__implies__value2Sterm_denotes; eauto.
+     
+        intros id' gv'0 HlookupEnv.
+        simpl.
+        destruct (id'==i0); subst.
+          exists (sterm_load (SMem sstate1) t (value2Sterm (STerms sstate1) v)).
+          split. 
+            apply binds_updateSmap_eq; auto.
+
+            apply lookupEnv_updateEnv_eq in H24; auto.
+            rewrite H24 in HlookupEnv.
+            inversion HlookupEnv; subst.
+            apply sterm_load_denotes with (Mem1:=Mem2)(gv0:=gv2)(mp0:=mp); eauto.
+              eapply genericvalue__implies__value2Sterm_denotes; eauto.
+
+          eapply se_cmd__denotes__op_cmd__case2; eauto.
+
+  Case "insn_store".
+    split; simpl.
+      destruct Hsterm_denotes as [J1 J2].
+      split; auto.
+    split; auto.
+      apply getOperandPtr_inversion in H24.
+      destruct H24 as [gv2 [J1 J2]].
+      eapply smem_store_denotes; 
+        eauto using genericvalue__implies__value2Sterm_denotes.
+
+  Case "insn_gep". 
+    split; auto.
+      split.
+        intros id' st' Hbinds.
+        simpl in Hbinds. simpl_env in Hbinds.
+        analyze_binds Hbinds.
+        apply updateSmap_inversion in Hbinds; auto.
+        apply getOperandPtr_inversion in H24.
+        destruct H24 as [gv0 [J1 J2]].
+        destruct Hbinds as [[nEQ Hbinds] | [EQ1 EQ2]]; subst.
+          eapply se_cmd__denotes__op_cmd__case1; eauto.
+
+          apply lookupEnv_updateEnv_eq in H26; auto.
+          rewrite H26.
+          apply GEP_inversion in H25.
+          destruct H25 as [idxs [J3 J4]].
+          apply intValues2Nats_inversion in J3.
+          destruct J3 as [gvs0 [J31 J32]].
+          exists (ptr2GV TD mp').
+          split; auto.
+            eapply sterm_gep_denotes; eauto using genericvalue__implies__value2Sterm_denotes, genericvalues__imply__value2Sterm_denote.
+
+        intros id' gv' HlookupEnv.
+        simpl. 
+        destruct (id'==i0); subst.
+          exists (sterm_gep i1 t (value2Sterm (STerms sstate1) v) (List.map (value2Sterm (STerms sstate1)) l0)).
+          split. 
+            apply binds_updateSmap_eq; auto.
+
+            apply lookupEnv_updateEnv_eq in H26; auto.
+            rewrite H26 in HlookupEnv.
+            inversion HlookupEnv; subst.
+            apply getOperandPtr_inversion in H24.
+            destruct H24 as [gv0 [J1 J2]].
+            apply GEP_inversion in H25.
+            destruct H25 as [idxs [J3 J4]].
+            apply intValues2Nats_inversion in J3.
+            destruct J3 as [gvs0 [J31 J32]].
+            eapply sterm_gep_denotes; eauto using genericvalue__implies__value2Sterm_denotes, genericvalues__imply__value2Sterm_denote.
+
+          eapply se_cmd__denotes__op_cmd__case2; eauto.
+
+  Case "insn_ext".
+    split; auto.
+      split.
+        intros id' st' Hbinds.
+        simpl in Hbinds. simpl_env in Hbinds.
+        analyze_binds Hbinds.
+        apply updateSmap_inversion in Hbinds; auto.
+        destruct Hbinds as [[nEQ Hbinds] | [EQ1 EQ2]]; subst.
+          eapply se_cmd__denotes__op_cmd__case1; eauto.
+
+          apply lookupEnv_updateEnv_eq in H25; auto.
+          rewrite H25.
+          apply EXT_inversion in H24.
+          destruct H24 as [gv1 [J1 J2]].
+          exists gv2. split; auto.
+            apply sterm_ext_denotes with (gv1:=gv1); eauto using genericvalue__implies__value2Sterm_denotes.
+
+        intros id' gv' HlookupEnv.
+        simpl. 
+        destruct (id'==i0); subst.
+          exists (sterm_ext e t (value2Sterm (STerms sstate1) v) t0).
+          split. 
+            apply binds_updateSmap_eq; auto.
+
+            apply lookupEnv_updateEnv_eq in H25; auto.
+            rewrite H25 in HlookupEnv.
+            inversion HlookupEnv; subst.
+            apply EXT_inversion in H24.
+            destruct H24 as [gv1 [J1 J2]].
+            apply sterm_ext_denotes with (gv1:=gv1); eauto using genericvalue__implies__value2Sterm_denotes.
+
+          eapply se_cmd__denotes__op_cmd__case2; eauto.
+
+  Case "insn_cast".
+    split; auto.
+      split.
+        intros id' st' Hbinds.
+        simpl in Hbinds. simpl_env in Hbinds.
+        analyze_binds Hbinds.
+        apply updateSmap_inversion in Hbinds; auto.
+        destruct Hbinds as [[nEQ Hbinds] | [EQ1 EQ2]]; subst.
+          eapply se_cmd__denotes__op_cmd__case1; eauto.
+
+          apply lookupEnv_updateEnv_eq in H25; auto.
+          rewrite H25.
+          apply CAST_inversion in H24.
+          destruct H24 as [gv1 [J1 J2]].
+          exists gv2. split; auto.
+            apply sterm_cast_denotes with (gv1:=gv1); eauto using genericvalue__implies__value2Sterm_denotes.
+
+        intros id' gv' HlookupEnv.
+        simpl. 
+        destruct (id'==i0); subst.
+          exists (sterm_cast c t (value2Sterm (STerms sstate1) v) t0).
+          split. 
+            apply binds_updateSmap_eq; auto.
+
+            apply lookupEnv_updateEnv_eq in H25; auto.
+            rewrite H25 in HlookupEnv.
+            inversion HlookupEnv; subst.
+            apply CAST_inversion in H24.
+            destruct H24 as [gv1 [J1 J2]].
+            apply sterm_cast_denotes with (gv1:=gv1); eauto using genericvalue__implies__value2Sterm_denotes.
+
+          eapply se_cmd__denotes__op_cmd__case2; eauto.
+
+  Case "insn_icmp".
+    split; auto.
+      split.
+        intros id' st' Hbinds.
+        simpl in Hbinds. simpl_env in Hbinds.
+        analyze_binds Hbinds.
+        apply updateSmap_inversion in Hbinds; auto.
+        destruct Hbinds as [[nEQ Hbinds] | [EQ1 EQ2]]; subst.
+          eapply se_cmd__denotes__op_cmd__case1; eauto.
+
+          apply lookupEnv_updateEnv_eq in H25; auto.
+          rewrite H25.
+          apply ICMP_inversion in H24.
+          destruct H24 as [gv1 [gv2 [J1 [J2 J3]]]].
+          exists gv3. split; auto.
+            apply sterm_icmp_denotes with (gv1:=gv1)(gv2:=gv2); eauto using genericvalue__implies__value2Sterm_denotes.
+
+        intros id' gv' HlookupEnv.
+        simpl. 
+        destruct (id'==i0); subst.
+          exists (sterm_icmp c t (value2Sterm (STerms sstate1) v) (value2Sterm (STerms sstate1) v0)).
+          split. 
+            apply binds_updateSmap_eq; auto.
+
+            apply lookupEnv_updateEnv_eq in H25; auto.
+            rewrite H25 in HlookupEnv.
+            inversion HlookupEnv; subst.
+            apply ICMP_inversion in H24.
+            destruct H24 as [gv1 [gv2 [J1 [J2 J3]]]].
+            apply sterm_icmp_denotes with (gv1:=gv1)(gv2:=gv2); eauto using genericvalue__implies__value2Sterm_denotes.
+
+          eapply se_cmd__denotes__op_cmd__case2; eauto.
+
+  Case "insn_select".
+    split; auto.
+      split.
+        intros id' st' Hbinds.
+        simpl in Hbinds. simpl_env in Hbinds.
+        analyze_binds Hbinds.
+        apply updateSmap_inversion in Hbinds; auto.
+        destruct Hbinds as [[nEQ Hbinds] | [EQ1 EQ2]]; subst.
+          destruct cond0; eapply se_cmd__denotes__op_cmd__case1; eauto.
+
+          symmetry in H27.
+          apply getOperandInt_inversion in H24. destruct H24 as [gv5 [J1 J2]].
+          destruct cond0; apply lookupEnv_updateEnv_eq in H27; auto.
+            exists gv1.
+            split; auto.
+              apply sterm_select_denotes with (c0:=0)(gv0:=gv5)(gv1:=gv1)(gv2:=gv2); eauto using genericvalue__implies__value2Sterm_denotes.
+
+            exists gv2.
+            split; auto.
+              apply sterm_select_denotes with (c0:=Datatypes.S cond0)(gv0:=gv5)(gv1:=gv1)(gv2:=gv2); eauto using genericvalue__implies__value2Sterm_denotes.
+
+        intros id' gv' HlookupEnv.
+        simpl. 
+        destruct (id'==i0); subst.
+          exists (sterm_select (value2Sterm (STerms sstate1) v) t (value2Sterm (STerms sstate1) v0) (value2Sterm (STerms sstate1) v1)).
+          split. 
+            apply binds_updateSmap_eq; auto.
+
+            apply getOperandInt_inversion in H24. destruct H24 as [gv5 [J1 J2]].
+            apply sterm_select_denotes with (c0:=cond0)(gv0:=gv5)(gv1:=gv1)(gv2:=gv2); eauto using genericvalue__implies__value2Sterm_denotes.
+            symmetry in H27.
+            destruct cond0;
+              apply lookupEnv_updateEnv_eq in H27; auto;
+              rewrite H27 in HlookupEnv;
+              inversion HlookupEnv; subst; auto.
+
+          destruct cond0; eapply se_cmd__denotes__op_cmd__case2; eauto.
+Qed.
+
+Lemma aux__op_cmds__satisfy__se_cmds : forall cs S TD Ps F B call0 sbs tmn lc0 arg als ECs gl0 als0 Mem0 lc als' gl Mem1 sstate1 lc' gl' Mem2 tr tr1,
+  dbCmds (mkState S TD Ps ((mkEC F B ((subblock_intro cs call0)::sbs) tmn lc arg als)::ECs) gl Mem1)
+         (mkState S TD Ps ((mkEC F B ((subblock_intro nil call0)::sbs) tmn lc' arg als')::ECs) gl' Mem2)
+         tr ->
+  uniq sstate1.(STerms) ->
+  (dom lc0 `union` dom gl0) [<=] dom (STerms sstate1) ->
+  sstate_denotes_state TD lc0 gl0 als0 Mem0 sstate1 lc gl als Mem1 tr1 ->
+  sstate_denotes_state TD lc0 gl0 als0 Mem0 (se_cmds sstate1 cs) lc' gl' als' Mem2 (trace_app tr1 tr).
+Proof.
+  induction cs; 
+    intros S TD Ps F B call0 sbs tmn lc0 arg0 als ECs gl0 als0 Mem0 lc als' gl Mem1 sstate1 lc' gl' Mem2 tr tr1 HdbCmds Huniq Hsub Hdenotes.
+
+    inversion HdbCmds; subst; try solve [rewrite trace_app_nil__eq__trace; auto].
+      inversion H.
+
+    inversion HdbCmds; subst.
+    assert (Hcmd:=H).
+    apply dbCmd_inversion in H.
+    destruct H as [lc3 [gl3 [als3 [Mem3 H]]]]; subst.
+    simpl.
+    apply op_cmd__satisfies__se_cmd with (lc0:=lc0)(gl0:=gl0)(sstate1:=sstate1)(als0:=als0)(Mem0:=Mem0)(tr1:=tr1) in Hcmd; auto.
+    rewrite trace_app_commute.
+    apply IHcs with (lc0:=lc0)(gl0:=gl0)(sstate1:=se_cmd sstate1 a)(als0:=als0)(Mem0:=Mem0)(tr1:=trace_app tr1 t1) in H0; auto.
+      apply se_cmd_uniq; auto.
+
+      destruct sstate1 as [smap1 sm1 sf1 se1].
+      assert (J:=@se_cmd_dom_mono smap1 sm1 sf1 se1 a).
+      clear - J Hsub. fsetdec.
+Qed.
+
+Lemma op_cmds__satisfy__se_cmds : forall S TD Ps F B cs call0 sbs tmn lc arg als ECs gl Mem lc' als' gl' Mem' tr,
+  uniq gl ->
+  uniq lc ->
+  dbCmds (mkState S TD Ps ((mkEC F B ((subblock_intro cs call0)::sbs) tmn lc arg als)::ECs) gl Mem)
+         (mkState S TD Ps ((mkEC F B ((subblock_intro nil call0)::sbs) tmn lc' arg als')::ECs) gl' Mem')
+         tr ->
+  sstate_denotes_state TD lc gl als Mem (se_cmds (mkSstate (env_to_smap gl lc) smem_init sframe_init nil) cs) lc' gl' als' Mem' tr.
+Proof.
+  intros S TD Ps F B cs call0 sbs tmn lc arg0 als ECs gl Mem0 lc' als' gl' Mem' tr Uniqg Uniqc HdbCmds.
+  apply aux__op_cmds__satisfy__se_cmds with (lc0:=lc)(gl0:=gl)(als0:=als)(Mem0:=Mem0)(sstate1:=mkSstate (env_to_smap gl lc) smem_init sframe_init nil) (tr1:=trace_nil) in HdbCmds; simpl; auto.
+    apply env_to_smap_uniq.
+    rewrite env_to_smap_dom_eq. fsetdec.
+    apply env_to_smap_denotes_id; auto.
+Qed.           
+
