src/TV/symexe_def.v
@@ -1,0 +1,1508 @@
+Add LoadPath "../ssa/ott".
+Add LoadPath "../ssa/monads".
+Add LoadPath "../ssa".
+Add LoadPath "../../../theory/metatheory".
+Require Import ssa.
+Require Import List.
+Require Export targetdata.
+Require Import monad.
+Require Import Arith.
+Require Import Metatheory.
+Require Import ssa_mem.
+Require Import genericvalues.
+Require Import ssa_dynamic.
+Require Import trace.
+
+(***************************************************************)
+(* Syntax easy to be proved with symbolic execution. *)
+
+Module SimpleSE.
+
+Inductive cmd : Set := 
+ | insn_bop : id -> bop -> sz -> value -> value -> cmd
+ | insn_extractvalue : id -> typ -> value -> list const -> cmd
+ | insn_insertvalue : id -> typ -> value -> typ -> value -> list const -> cmd
+ | insn_malloc : id -> typ -> sz -> align -> cmd
+ | insn_free : id -> typ -> value -> cmd
+ | insn_alloca : id -> typ -> sz -> align -> cmd
+ | insn_load : id -> typ -> value -> cmd
+ | insn_store : id -> typ -> value -> value -> cmd
+ | insn_gep : id -> inbounds -> typ -> value -> list value -> cmd
+ | insn_ext : id -> extop -> typ -> value -> typ -> cmd
+ | insn_cast : id -> castop -> typ -> value -> typ -> cmd
+ | insn_icmp : id -> cond -> typ -> value -> value -> cmd
+ | insn_select : id -> value -> typ -> value -> value -> cmd
+.
+
+Tactic Notation "cmd_cases" tactic(first) tactic(c) :=
+  first;
+  [ c "insn_bop" | c "insn_extractvalue" | c "insn_insertvalue" |
+    c "insn_malloc" | c "insn_free" |
+    c "insn_alloca" | c "insn_load" | c "insn_store" | c "insn_gep" |
+    c "insn_ext" | c "insn_cast" | c "insn_icmp" |  c "insn_select" ].
+
+Inductive call : Set := 
+ | insn_call : id -> noret -> tailc -> typ -> id -> list_param -> call.
+
+Inductive subblock : Set :=
+ | subblock_intro : list cmd -> call -> subblock.
+
+Inductive block : Set :=
+ | block_intro : l -> list phinode -> list subblock -> terminator -> block.
+
+Inductive fdef : Set := 
+ | fdef_intro : fheader -> list block -> fdef.
+
+Inductive product : Set := 
+ | product_gvar : gvar -> product
+ | product_fdec : fdec -> product
+ | product_fdef : fdef -> product.
+
+Inductive module : Set := 
+ | module_intro : list_layout -> list product -> module.
+
+Definition system : Set := list module.
+
+(***************************************************************)
+(* deterministic big-step for this new syntax with subblocks. *)
+
+Record ExecutionContext : Set := mkEC {
+CurFunction : fdef;
+CurBB       : block;
+CurCmds     : list subblock;         (* subblock to run within CurBB *)
+Terminator  : terminator;
+Locals      : GVMap;                 (* LLVM values used in this invocation *)
+Args        : list GenericValue;      
+Allocas     : list mblock            (* Track memory allocated by alloca *)
+}.
+
+Definition ECStack := list ExecutionContext.
+
+Record State : Set := mkState {
+CurSystem      : system;
+CurTatgetData  : layouts;
+CurProducts    : list product;
+ECS            : ECStack;
+Globals        : GVMap;
+Mem            : mem
+}.
+
+Variable lookupBlockViaLabelFromSystem : system -> l -> option block.
+Variable switchToNewBasicBlock : block -> block -> GVMap -> GVMap.
+Variable lookupFdefViaIDFromSystem : system -> id -> option fdef.
+Variable getEntryBlock : fdef -> option block.
+
+Inductive dbCmd : State -> State -> trace -> Prop :=
+| dbBop: forall S TD Ps F B lc gl lc' gl' arg id bop sz v1 v2 gv3 EC cs c sbs tmn Mem als,
+  BOP TD lc gl bop sz v1 v2 = Some gv3 ->
+  updateEnv lc gl id gv3 = (lc', gl') -> 
+  dbCmd 
+    (mkState S TD Ps ((mkEC F B ((subblock_intro ((insn_bop id bop sz v1 v2)::cs) c)::sbs) tmn lc arg als)::EC) gl Mem) 
+    (mkState S TD Ps ((mkEC F B ((subblock_intro cs c)::sbs) tmn lc' arg als)::EC) gl' Mem)
+    trace_nil 
+| dbExtractValue : forall S TD Ps F B lc gl lc' gl' arg id t v gv gv' idxs EC cs c sbs tmn Mem als,
+  getOperandValue TD v lc gl = Some gv ->
+  extractGenericValue TD t gv idxs = Some gv' ->
+  updateEnv lc gl id gv' = (lc', gl') -> 
+  dbCmd 
+    (mkState S TD Ps ((mkEC F B ((subblock_intro ((insn_extractvalue id t v idxs)::cs) c)::sbs) tmn lc arg als)::EC) gl Mem) 
+    (mkState S TD Ps ((mkEC F B ((subblock_intro cs c)::sbs) tmn lc' arg als)::EC) gl' Mem)
+    trace_nil 
+| dbInsertValue : forall S TD Ps F B lc gl lc' gl' arg id t v t' v' gv gv' gv'' idxs EC cs c sbs tmn Mem als,
+  getOperandValue TD v lc gl = Some gv ->
+  getOperandValue TD v' lc gl = Some gv' ->
+  insertGenericValue TD t gv idxs t' gv' = Some gv'' ->
+  updateEnv lc gl id gv'' = (lc', gl') -> 
+  dbCmd 
+    (mkState S TD Ps ((mkEC F B ((subblock_intro ((insn_insertvalue id t v t' v' idxs)::cs) c)::sbs) tmn lc arg als)::EC) gl Mem) 
+    (mkState S TD Ps ((mkEC F B ((subblock_intro cs c)::sbs) tmn lc' arg als)::EC) gl' Mem)
+    trace_nil 
+| dbMalloc : forall S TD Ps F B lc gl lc' gl' arg id t sz align EC cs c sbs tmn Mem als Mem' tsz mb,
+  getTypeAllocSize TD t = Some tsz ->
+  malloc TD Mem (tsz * sz) align = Some (Mem', mb) ->
+  updateEnv lc gl id (ptr2GV TD (mb, 0)) = (lc', gl') -> 
+  dbCmd 
+    (mkState S TD Ps ((mkEC F B ((subblock_intro ((insn_malloc id t sz align)::cs) c)::sbs) tmn lc arg als)::EC) gl Mem) 
+    (mkState S TD Ps ((mkEC F B ((subblock_intro cs c)::sbs) tmn lc' arg als)::EC) gl' Mem')
+    trace_nil
+| dbFree : forall S TD Ps F B lc gl arg fid t v EC cs c sbs tmn Mem als Mem' mptr,
+  getOperandPtr TD v lc gl = Some mptr ->
+  free Mem mptr = Some Mem'->
+  dbCmd 
+    (mkState S TD Ps ((mkEC F B ((subblock_intro ((insn_free fid t v)::cs) c)::sbs) tmn lc arg als)::EC) gl Mem) 
+    (mkState S TD Ps ((mkEC F B ((subblock_intro cs c)::sbs) tmn lc arg als)::EC) gl Mem')
+    trace_nil
+| dbAlloca : forall S TD Ps F B lc gl lc' gl' arg id t sz align EC cs c sbs tmn Mem als Mem' tsz mb,
+  getTypeAllocSize TD t = Some tsz ->
+  malloc TD Mem (tsz * sz) align = Some (Mem', mb) ->
+  updateEnv lc gl id (ptr2GV TD (mb, 0)) = (lc', gl') -> 
+  dbCmd 
+    (mkState S TD Ps ((mkEC F B ((subblock_intro ((insn_alloca id t sz align)::cs) c)::sbs) tmn lc arg als)::EC) gl Mem) 
+    (mkState S TD Ps ((mkEC F B ((subblock_intro cs c)::sbs) tmn lc' arg (mb::als))::EC) gl' Mem')
+    trace_nil
+| dbLoad : forall S TD Ps F B lc gl lc' gl' arg id t v EC cs c sbs tmn Mem als mp gv,
+  getOperandPtr TD v lc gl = Some mp ->
+  mload TD Mem mp t = Some gv ->
+  updateEnv lc gl id gv = (lc', gl') -> 
+  dbCmd 
+    (mkState S TD Ps ((mkEC F B ((subblock_intro ((insn_load id t v)::cs) c)::sbs) tmn lc arg als)::EC) gl Mem) 
+    (mkState S TD Ps ((mkEC F B ((subblock_intro cs c)::sbs) tmn lc' arg als)::EC) gl' Mem)
+    trace_nil
+| dbStore : forall S TD Ps F B lc gl arg sid t v1 v2 EC cs c sbs tmn Mem als mp2 gv1 Mem',
+  getOperandValue TD v1 lc gl = Some gv1 ->
+  getOperandPtr TD v2 lc gl = Some mp2 ->
+  mstore TD Mem mp2 t gv1 = Some Mem' ->
+  dbCmd 
+    (mkState S TD Ps ((mkEC F B ((subblock_intro ((insn_store sid t v1 v2)::cs) c)::sbs) tmn lc arg als)::EC) gl Mem) 
+    (mkState S TD Ps ((mkEC F B ((subblock_intro cs c)::sbs) tmn lc arg als)::EC) gl Mem')
+    trace_nil
+| dbGEP : forall S TD Ps F B lc gl lc' gl' arg id inbounds t v idxs EC mp mp' cs c sbs tmn Mem als,
+  getOperandPtr TD v lc gl = Some mp ->
+  GEP TD lc gl t mp idxs inbounds = Some mp' ->
+  updateEnv lc gl id (ptr2GV TD mp') = (lc', gl') -> 
+  dbCmd 
+    (mkState S TD Ps ((mkEC F B ((subblock_intro ((insn_gep id inbounds t v idxs)::cs) c)::sbs) tmn lc arg als)::EC) gl Mem) 
+    (mkState S TD Ps ((mkEC F B ((subblock_intro cs c)::sbs) tmn lc' arg als)::EC) gl' Mem)
+    trace_nil 
+| dbExt : forall S TD Ps F B lc gl arg id extop t1 v1 t2 gv2 EC cs c sbs tmn lc' gl' Mem als,
+  EXT TD lc gl extop t1 v1 t2 = Some gv2 ->
+  updateEnv lc gl id gv2 = (lc', gl') -> 
+  dbCmd 
+    (mkState S TD Ps ((mkEC F B ((subblock_intro ((insn_ext id extop t1 v1 t2)::cs) c)::sbs) tmn lc arg als)::EC) gl Mem) 
+    (mkState S TD Ps ((mkEC F B ((subblock_intro cs c)::sbs) tmn lc' arg als)::EC) gl' Mem)
+    trace_nil
+| dbCast : forall S TD Ps F B lc gl arg id castop t1 v1 t2 gv2 EC cs c sbs tmn lc' gl' Mem als,
+  CAST TD lc gl castop t1 v1 t2 = Some gv2 ->
+  updateEnv lc gl id gv2 = (lc', gl') -> 
+  dbCmd 
+    (mkState S TD Ps ((mkEC F B ((subblock_intro ((insn_cast id castop t1 v1 t2)::cs) c)::sbs) tmn lc arg als)::EC) gl Mem) 
+    (mkState S TD Ps ((mkEC F B ((subblock_intro cs c)::sbs) tmn lc' arg als)::EC) gl' Mem)
+    trace_nil
+| dbIcmp : forall S TD Ps F B lc gl arg id cond t v1 v2 gv3 EC cs c sbs tmn lc' gl' Mem als,
+  ICMP TD lc gl cond t v1 v2 = Some gv3 ->
+  updateEnv lc gl id gv3 = (lc', gl') -> 
+  dbCmd 
+    (mkState S TD Ps ((mkEC F B ((subblock_intro ((insn_icmp id cond t v1 v2)::cs) c)::sbs) tmn lc arg als)::EC) gl Mem) 
+    (mkState S TD Ps ((mkEC F B ((subblock_intro cs c)::sbs) tmn lc' arg als)::EC) gl' Mem)
+    trace_nil
+| dbSelect : forall S TD Ps F B lc gl arg id v0 t v1 v2 cond EC cs c sbs tmn lc' gl' Mem als gv1 gv2,
+  getOperandInt TD 1 v0 lc gl = Some cond ->
+  getOperandValue TD v1 lc gl = Some gv1 ->
+  getOperandValue TD v2 lc gl = Some gv2 ->
+  (lc', gl') = (if cond
+               then updateEnv lc gl id gv1
+               else updateEnv lc gl id gv2) ->
+  dbCmd 
+    (mkState S TD Ps ((mkEC F B ((subblock_intro ((insn_select id v0 t v1 v2)::cs) c)::sbs) tmn lc arg als)::EC) gl Mem) 
+    (mkState S TD Ps ((mkEC F B ((subblock_intro cs c)::sbs) tmn lc' arg als)::EC) gl' Mem)
+    trace_nil
+.
+
+Inductive dbTerminator : State -> State -> trace -> Prop :=
+| dbBranch : forall S TD Ps F B lc gl arg bid Cond l1 l2 c
+                              l' ps' sbs' tmn' lc' EC Mem als,   
+  getOperandInt TD 1 Cond lc gl = Some c ->
+  Some (block_intro l' ps' sbs' tmn') = (if c 
+               then lookupBlockViaLabelFromSystem S l1
+               else lookupBlockViaLabelFromSystem S l2) ->
+  lc' = switchToNewBasicBlock (block_intro l' ps' sbs' tmn') B lc ->
+  dbTerminator 
+    (mkState S TD Ps ((mkEC F B nil (insn_br bid Cond l1 l2) lc arg als)::EC) gl Mem)
+    (mkState S TD Ps ((mkEC F (block_intro l' ps' sbs' tmn') sbs' tmn' lc' arg als)::EC) gl Mem)
+    trace_nil 
+| dbBranch_uncond : forall S TD Ps F B lc gl arg l bid
+                              l' ps' sbs' tmn' lc' EC Mem als,   
+  Some (block_intro l' ps' sbs' tmn') = (lookupBlockViaLabelFromSystem S l) ->
+  lc' = switchToNewBasicBlock (block_intro l' ps' sbs' tmn') B lc ->
+  dbTerminator 
+    (mkState S TD Ps ((mkEC F B nil (insn_br_uncond bid l) lc arg als)::EC) gl Mem)
+    (mkState S TD Ps ((mkEC F (block_intro l' ps' sbs' tmn') sbs' tmn' lc' arg als)::EC) gl Mem)
+    trace_nil 
+.
+
+Inductive dbCmds : State -> State -> trace -> Prop :=
+| dbCmds_nil : forall S, dbCmds S S trace_nil
+| dbCmds_cons : forall S1 S2 S3 t1 t2,
+    dbCmd S1 S2 t1 ->
+    dbCmds S2 S3 t2 ->
+    dbCmds S1 S3 (trace_app t1 t2).
+
+Inductive dbCall : State -> State -> trace -> Prop :=
+| dbCall_intro : forall S TD Ps F B lc gl arg rid noret tailc rt fid lp gl' gl'' sbs tmn
+                       EC Rid oResult tr lc'' B' lc' Mem Mem' als' als Mem'',
+  dbFdef fid rt lp S TD Ps ((mkEC F B ((subblock_intro nil (insn_call rid noret tailc rt fid lp))::sbs) tmn lc arg als)::EC) lc gl Mem lc' gl' als' Mem' B' Rid oResult tr ->
+  (lc'', gl'') = 
+    match noret with
+    | false =>
+      if (LLVMlib.typEqB rt typ_void) 
+      then (lc, gl') 
+      else 
+        match oResult with
+        | None => (lc, gl')
+        | Some Result => 
+          match (getOperandValue TD Result lc' gl') with
+          | Some gr => updateEnv lc gl' rid gr
+          | None => (lc, gl')
+          end
+        end
+    | true => (lc, gl')
+    end ->
+  free_allocas Mem' als' = Some Mem'' ->
+  dbCall 
+    (mkState S TD Ps ((mkEC F B ((subblock_intro nil (insn_call rid noret tailc rt fid lp))::sbs) tmn lc arg als)::EC) gl Mem) 
+    (mkState S TD Ps ((mkEC F B sbs tmn lc'' arg als)::EC) gl'' Mem'') 
+    tr
+with dbSubblock : State -> State -> trace -> Prop :=
+| dbSubblock_intro : forall state1 state2 tr1 state3 tr2,
+  dbCmds state1 state2 tr1 ->
+  dbCall state2 state3 tr2 ->
+  dbSubblock state1 state3 (trace_app tr1 tr2)
+with dbSubblocks : State -> State -> trace -> Prop :=
+| dbSubblocks_nil : forall S, dbSubblocks S S trace_nil
+| dbSubblocks_cond : forall S1 S2 S3 t1 t2,
+    dbSubblock S1 S2 t1 ->
+    dbSubblocks S2 S3 t2 ->
+    dbSubblocks S1 S3 (trace_app t1 t2)
+with dbBlock : State -> State -> trace -> Prop :=
+| dbBlock_intro : forall state1 state2 tr1 state3 tr2,
+  dbSubblocks state1 state2 tr1 ->
+  dbTerminator state2 state3 tr2 ->
+  dbBlock state1 state3 (trace_app tr1 tr2)
+with dbBlocks : State -> State -> trace -> Prop :=
+| dbBlocks_nil : forall S, dbBlocks S S trace_nil
+| dbBlocks_cons : forall S1 S2 S3 t1 t2,
+    dbBlock S1 S2 t1 ->
+    dbBlocks S2 S3 t2 ->
+    dbBlocks S1 S3 (trace_app t1 t2)
+with dbFdef : id -> typ -> list_param -> system -> layouts -> list product -> list ExecutionContext -> GVMap -> GVMap -> mem -> GVMap -> GVMap -> list mblock -> mem -> block -> id -> option value -> trace -> Prop :=
+| dbFdef_func : forall S TD Ps gl fid lp lc rid
+                            l' ps' cs' tmn' rt la lb B'' Result lc' gl' tr ECs Mem Mem' als',
+  lookupFdefViaIDFromSystem S fid = Some (fdef_intro (fheader_intro rt fid la) lb) ->
+  getEntryBlock (fdef_intro (fheader_intro rt fid la) lb) = Some (block_intro l' ps' cs' tmn') ->
+  dbBlocks 
+    (mkState S TD Ps ((mkEC (fdef_intro (fheader_intro rt fid la) lb) 
+                             (block_intro l' ps' cs' tmn') cs' tmn' (initLocals la (params2GVs TD lp lc gl))
+                            (params2GVs TD lp lc gl) nil)::ECs) gl Mem)
+    (mkState S TD Ps ((mkEC (fdef_intro (fheader_intro rt fid la) lb) 
+                             B'' nil (insn_return rid rt Result) lc'
+                            (params2GVs TD lp lc gl) als')::ECs) gl' Mem')
+    tr ->
+  dbFdef fid rt lp S TD Ps ECs lc gl Mem lc' gl' als' Mem' B'' rid (Some Result) tr
+| dbFdef_proc : forall S TD Ps gl fid lp lc rid
+                            l' ps' cs' tmn' rt la lb B'' lc' gl' tr ECs Mem Mem' als',
+  lookupFdefViaIDFromSystem S fid = Some (fdef_intro (fheader_intro rt fid la) lb) ->
+  getEntryBlock (fdef_intro (fheader_intro rt fid la) lb) = Some (block_intro l' ps' cs' tmn') ->
+  dbBlocks 
+    (mkState S TD Ps ((mkEC (fdef_intro (fheader_intro rt fid la) lb) 
+                             (block_intro l' ps' cs' tmn') cs' tmn' (initLocals la (params2GVs TD lp lc gl))
+                            (params2GVs TD lp lc gl) nil)::ECs) gl Mem)
+    (mkState S TD Ps ((mkEC (fdef_intro (fheader_intro rt fid la) lb) 
+                             B'' nil (insn_return_void rid) lc'
+                            (params2GVs TD lp lc gl) als')::ECs) gl' Mem')
+    tr ->
+  dbFdef fid  rt lp S TD Ps ECs lc gl Mem lc' gl' als' Mem' B'' rid None tr
+.
+
+Scheme dbCall_ind2 := Induction for dbCall Sort Prop
+  with dbSubblock_ind2 := Induction for dbSubblock Sort Prop
+  with dbSubblocks_ind2 := Induction for dbSubblocks Sort Prop
+  with dbBlock_ind2 := Induction for dbBlock Sort Prop
+  with dbBlocks_ind2 := Induction for dbBlocks Sort Prop
+  with dbFdef_ind2 := Induction for dbFdef Sort Prop.
+
+Combined Scheme db_mutind from dbCall_ind2, dbSubblock_ind2, dbSubblocks_ind2,
+                               dbBlock_ind2, dbBlocks_ind2, dbFdef_ind2.
+
+Tactic Notation "db_mutind_cases" tactic(first) tactic(c) :=
+  first;
+  [ c "dbCall_intro" | 
+    c "dbSubblock_intro" | c "dbSubblocks_nil" | c "dbSubblocks_cons" | 
+    c "dbBlock_intro" | c "dbBlocks_nil" | c "dbBlocks_cons" | 
+    c "dbFdef_func" | c "dbFdef_proc" ].
+
+Tactic Notation "dbCmd_cases" tactic(first) tactic(c) :=
+  first;
+  [ c "dbBop" | c "dbExtractValue" | c "dbInsertValue" |
+    c "dbMalloc" | c "dbFree" |
+    c "dbAlloca" | c "dbLoad" | c "dbStore" | c "dbGEP" |
+    c "dbExt" | c "dbCast" | c "dbIcmp" |  c "dbSelect" ].
+
+Tactic Notation "dbTerminator_cases" tactic(first) tactic(c) :=
+  first;
+  [ c "dbBranch" | c "dbBranch_uncond" ].
+
+Tactic Notation "dbCmds_cases" tactic(first) tactic(c) :=
+  first;
+  [ c "dbCmds_nil" | c "dbCmds_cons" ].
+
+Hint Constructors dbCmd dbCmds dbTerminator dbCall 
+                  dbSubblock dbSubblocks dbBlock dbBlocks dbFdef.
+
+(* properties of opsem *)
+Lemma dbCmd_inversion : forall a cs S TD Ps F B call0 sbs tmn arg als ECs lc gl Mem1 state2 tr,
+  dbCmd (mkState S TD Ps ((mkEC F B ((subblock_intro (a::cs) call0)::sbs) tmn lc arg als)::ECs) gl Mem1)
+        state2
+        tr ->
+  exists lc', exists gl', exists als', exists Mem2,
+    state2 = (mkState S TD Ps ((mkEC F B ((subblock_intro cs call0)::sbs) tmn lc' arg als')::ECs) gl' Mem2).
+Proof.
+  intros a cs S TD Ps F B call0 sbs tmn arg0 als ECs lc gl Mem1 state2 tr HdbCmd.
+  inversion HdbCmd; subst; 
+  try solve [
+    exists lc'; exists gl'; exists als; exists Mem1; auto |
+    exists lc'; exists gl'; exists als; exists Mem'; auto |
+    exists lc; exists gl; exists als; exists Mem'; auto |
+    exists lc'; exists gl'; exists (mb::als); exists Mem'; auto
+  ].
+Qed.
+
+Lemma dbCmd_eqEnv : forall S TD Ps F B c cs cs' call0 sbs tmn lc1 arg als1 ECs gl1 Mem1 lc2 als2 gl2 Mem2 tr lc2' gl2',
+  dbCmd (mkState S TD Ps ((mkEC F B ((subblock_intro (c::cs) call0)::sbs) tmn lc1 arg als1)::ECs) gl1 Mem1)
+        (mkState S TD Ps ((mkEC F B ((subblock_intro cs' call0)::sbs) tmn lc2 arg als2)::ECs) gl2 Mem2)
+        tr ->
+  eqEnv lc2 gl2 lc2' gl2' ->
+  dbCmd (mkState S TD Ps ((mkEC F B ((subblock_intro (c::cs) call0)::sbs) tmn lc1 arg als1)::ECs) gl1 Mem1)
+        (mkState S TD Ps ((mkEC F B ((subblock_intro cs' call0)::sbs) tmn lc2' arg als2)::ECs) gl2' Mem2)
+        tr.
+Admitted.
+
+Lemma dbCmds_eqEnv : forall S TD Ps F B cs cs' call0 sbs tmn lc1 arg als1 ECs gl1 Mem1 lc2 als2 gl2 Mem2 tr lc2' gl2',
+  dbCmds (mkState S TD Ps ((mkEC F B ((subblock_intro cs call0)::sbs) tmn lc1 arg als1)::ECs) gl1 Mem1)
+        (mkState S TD Ps ((mkEC F B ((subblock_intro cs' call0)::sbs) tmn lc2 arg als2)::ECs) gl2 Mem2)
+        tr ->
+  eqEnv lc2 gl2 lc2' gl2' ->
+  dbCmds (mkState S TD Ps ((mkEC F B ((subblock_intro cs call0)::sbs) tmn lc1 arg als1)::ECs) gl1 Mem1)
+        (mkState S TD Ps ((mkEC F B ((subblock_intro cs' call0)::sbs) tmn lc2' arg als2)::ECs) gl2' Mem2)
+        tr.
+Admitted.
+
+Lemma dbCmds_uniq : forall S TD Ps F B cs cs' call0 sbs tmn lc1 arg als1 ECs gl1 Mem1 lc2 als2 gl2 Mem2 tr,
+  uniq gl1 ->
+  uniq lc1 ->
+  dbCmds (mkState S TD Ps ((mkEC F B ((subblock_intro cs call0)::sbs) tmn lc1 arg als1)::ECs) gl1 Mem1)
+        (mkState S TD Ps ((mkEC F B ((subblock_intro cs' call0)::sbs) tmn lc2 arg als2)::ECs) gl2 Mem2)
+        tr ->
+  uniq gl2 /\ uniq lc2.
+Admitted.
+
+(***************************************************************)
+(** symbolic terms and memories. *)
+Inductive sterm : Set := 
+| sterm_val : value -> sterm
+| sterm_bop : bop -> sz -> sterm -> sterm -> sterm
+| sterm_extractvalue : typ -> sterm -> list const -> sterm
+| sterm_insertvalue : typ -> sterm -> typ -> sterm -> list const -> sterm
+| sterm_malloc : smem -> typ -> sz -> align -> sterm
+| sterm_alloca : smem -> typ -> sz -> align -> sterm
+| sterm_load : smem -> typ -> sterm -> sterm
+| sterm_gep : inbounds -> typ -> sterm -> list sterm -> sterm
+| sterm_ext : extop -> typ -> sterm -> typ -> sterm
+| sterm_cast : castop -> typ -> sterm -> typ -> sterm
+| sterm_icmp : cond -> typ -> sterm -> sterm -> sterm
+| sterm_phi : typ -> list (sterm*l) -> sterm
+| sterm_select : sterm -> typ -> sterm -> sterm -> sterm
+with smem : Set :=
+| smem_init : smem
+| smem_malloc : smem -> typ -> sz -> align -> smem
+| smem_free : smem -> typ -> sterm -> smem
+| smem_alloca : smem -> typ -> sz -> align -> smem
+| smem_load : smem -> typ -> sterm -> smem
+| smem_store : smem -> typ -> sterm -> sterm -> smem
+with sframe : Set :=
+| sframe_init : sframe
+| sframe_alloca : smem -> sframe -> typ -> sz -> align -> sframe
+.
+
+Inductive sterminator : Set :=
+| stmn_return : id -> typ -> sterm -> sterminator
+| stmn_return_void : id -> sterminator
+| stmn_br : id -> sterm -> l -> l -> sterminator
+| stmn_br_uncond : id -> l -> sterminator
+| stmn_unreachable : id -> sterminator
+.
+
+Inductive scall : Set :=
+| stmn_call : id -> noret -> tailc -> typ -> id -> list (typ*sterm) -> scall
+.
+
+Definition smap := list (atom*sterm).
+
+Record sstate : Set := mkSstate 
+{
+  STerms : smap;
+  SMem : smem;
+  SFrame : sframe;
+  SEffects : list sterm
+}.
+
+Fixpoint updateSmap (sm:smap) (id0:id) (s0:sterm) : smap :=
+match sm with
+| nil => (id0, s0)::nil
+| (id1, s1)::sm' =>
+  if id1==id0
+  then (id1, s0)::sm'
+  else (id1, s1)::updateSmap sm' id0 s0
+end.
+
+Fixpoint lookupSmap (sm:smap) (i0:id) : sterm :=
+match sm with
+| nil => (sterm_val (value_id i0))
+| (id0, s0)::sm' => 
+  if id0 == i0 then s0 else lookupSmap sm' i0
+end.
+
+Definition value2Sterm (sm:smap) (v:value) : sterm :=
+match v with
+| value_const _ => sterm_val v
+| value_id i0 => lookupSmap sm i0
+end.
+
+Fixpoint list_param__list_typ_subst_sterm (list_param1:list_param) (sm:smap) : list (typ*sterm) :=
+match list_param1 with
+| nil => nil
+| (t, v)::list_param1' => (t, (value2Sterm sm v))::(list_param__list_typ_subst_sterm list_param1' sm)
+end.
+
+Definition se_cmd (st : sstate) (i:cmd) : sstate :=
+match i with 
+| insn_bop id0 op0 sz0 v1 v2 => 
+       (mkSstate (updateSmap st.(STerms) id0 
+                   (sterm_bop op0 sz0 
+                     (value2Sterm st.(STerms) v1)
+                     (value2Sterm st.(STerms) v2)))
+                 st.(SMem)
+                 st.(SFrame)
+                 st.(SEffects))
+| insn_extractvalue id0 t1 v1 cs3 =>
+       (mkSstate (updateSmap st.(STerms) id0 
+                   (sterm_extractvalue t1 
+                     (value2Sterm st.(STerms) v1)
+                     cs3))
+                 st.(SMem)
+                 st.(SFrame)
+                 st.(SEffects))
+| insn_insertvalue id0 t1 v1 t2 v2 cs3 =>  
+       (mkSstate (updateSmap st.(STerms) id0 
+                   (sterm_insertvalue 
+                     t1 
+                     (value2Sterm st.(STerms) v1)
+                     t2 
+                     (value2Sterm st.(STerms) v2)
+                     cs3))
+                 st.(SMem)
+                 st.(SFrame)
+                 st.(SEffects))
+| insn_malloc id0 t1 sz1 al1 =>  
+       (mkSstate (updateSmap st.(STerms) id0 
+                   (sterm_malloc st.(SMem) t1 sz1 al1))
+                 (smem_malloc st.(SMem) t1 sz1 al1)
+                 st.(SFrame)
+                 st.(SEffects))
+| insn_free id0 t0 v0 =>  
+       (mkSstate st.(STerms)
+                 (smem_free st.(SMem) t0 
+                   (value2Sterm st.(STerms) v0))
+                 st.(SFrame)
+                 st.(SEffects))
+| insn_alloca id0 t1 sz1 al1 =>  
+       (mkSstate (updateSmap st.(STerms) id0 
+                   (sterm_alloca st.(SMem) t1 sz1 al1))
+                 (smem_alloca st.(SMem) t1 sz1 al1)
+                 (sframe_alloca st.(SMem) st.(SFrame) t1 sz1 al1)
+                 st.(SEffects))
+| insn_load id0 t2 v2 =>  
+       (mkSstate (updateSmap st.(STerms) id0 
+                   (sterm_load st.(SMem) t2 
+                     (value2Sterm st.(STerms) v2)))
+                 (smem_load st.(SMem)t2 
+                   (value2Sterm st.(STerms) v2))
+                 st.(SFrame)
+                 st.(SEffects))
+| insn_store id0 t0 v1 v2 =>  
+       (mkSstate st.(STerms)
+                 (smem_store st.(SMem) t0 
+                   (value2Sterm st.(STerms) v1)
+                   (value2Sterm st.(STerms) v2))
+                 st.(SFrame)
+                 st.(SEffects))
+| insn_gep id0 inbounds0 t1 v1 lv2 =>  
+       (mkSstate (updateSmap st.(STerms) id0 
+                   (sterm_gep inbounds0 t1 
+                     (value2Sterm st.(STerms) v1)
+                     (List.map (value2Sterm st.(STerms)) lv2)))
+                 st.(SMem)
+                 st.(SFrame)
+                 st.(SEffects))
+| insn_ext id0 op0 t1 v1 t2 =>  
+       (mkSstate (updateSmap st.(STerms) id0 
+                   (sterm_ext op0 t1 
+                     (value2Sterm st.(STerms) v1)
+                     t2))
+                 st.(SMem)
+                 st.(SFrame)
+                 st.(SEffects))
+| insn_cast id0 op0 t1 v1 t2 =>  
+       (mkSstate (updateSmap st.(STerms) id0 
+                   (sterm_cast op0 t1 
+                     (value2Sterm st.(STerms) v1)
+                     t2))
+                 st.(SMem)
+                 st.(SFrame)
+                 st.(SEffects))
+| insn_icmp id0 c0 t0 v1 v2 =>  
+       (mkSstate (updateSmap st.(STerms) id0 
+                   (sterm_icmp c0 t0 
+                     (value2Sterm st.(STerms) v1)
+                     (value2Sterm st.(STerms) v2)))
+                 st.(SMem)
+                 st.(SFrame)
+                 st.(SEffects))
+| insn_select id0 v0 t0 v1 v2 =>  
+       (mkSstate (updateSmap st.(STerms) id0 
+                   (sterm_select 
+                     (value2Sterm st.(STerms) v0)
+                     t0 
+                     (value2Sterm st.(STerms) v1)
+                     (value2Sterm st.(STerms) v2)))
+                 st.(SMem)
+                 st.(SFrame)
+                 st.(SEffects))
+end.
+
+Fixpoint _se_phinodes (st st0: sstate) (ps:list phinode) : sstate :=
+match ps with
+| nil => st
+| insn_phi id0 t0 idls0::ps' =>  
+    _se_phinodes 
+     (mkSstate (updateSmap st.(STerms) id0 
+                 (sterm_phi 
+                   t0 
+                   (List.map
+                     (fun (idl:id*l) =>
+                      let (id5, l5) := idl in
+                      ((value2Sterm st.(STerms) (value_id id5)), l5)
+                     )
+                     idls0
+                   )
+                 )
+               )
+               st.(SMem)
+               st.(SFrame)
+               st.(SEffects))
+     st0
+     ps'
+end.
+
+Fixpoint se_phinodes (st: sstate) (ps:list phinode) := _se_phinodes st st ps.
+
+Fixpoint se_cmds (st : sstate) (cs:list cmd) : sstate :=
+match cs with
+| nil => st
+| c::cs' => se_cmds (se_cmd st c) cs'
+end.
+
+Definition se_terminator (st : sstate) (i:terminator) : sterminator :=
+match i with 
+| insn_return id0 t0 v0 => stmn_return id0 t0 (value2Sterm st.(STerms) v0)
+| insn_return_void id0 => stmn_return_void id0 
+| insn_br id0 v0 l1 l2 => stmn_br id0 (value2Sterm st.(STerms) v0) l1 l2
+| insn_br_uncond id0 l0 => stmn_br_uncond id0 l0
+| insn_unreachable id0 => stmn_unreachable id0 
+end.
+
+Definition se_call (st : sstate) (i:call) : scall :=
+match i with
+| insn_call id0 noret tailc0 t1 id1 list_param1 =>  
+                   (stmn_call id0 noret tailc0 t1 id1 
+                      (list_param__list_typ_subst_sterm list_param1 st.(STerms)))
+end.
+
+(* Properties *)
+
+Lemma updateSmap_dom_eq : forall sm id0 st0,
+  dom (updateSmap sm id0 st0) [=] dom sm `union` {{id0}}.
+Proof.
+  induction sm; intros; simpl; try solve [fsetdec].
+    destruct a. 
+    destruct (a==id0); simpl; try solve [fsetdec].
+      assert (J:=@IHsm id0 st0). fsetdec.
+Qed.
+
+Lemma updateSmap_uniq : forall sm id0 st0,
+  uniq sm ->
+  uniq (updateSmap sm id0 st0).
+Proof.
+  induction sm; intros; simpl; auto.
+    destruct a.
+
+    destruct_uniq.
+    destruct (a==id0); subst; try solve [solve_uniq].
+      apply IHsm with (id0:=id0)(st0:=st0) in H. 
+      assert (J:=@updateSmap_dom_eq sm id0 st0).
+      solve_uniq.
+Qed.
+
+Lemma se_cmd_uniq : forall smap0 sm0 sf0 se0 c,
+  uniq smap0 ->
+  uniq (STerms (se_cmd (mkSstate smap0 sm0 sf0 se0) c)).
+Proof.
+  intros smap0 sm0 sf0 se0 c Huniq.
+  destruct c; simpl; try solve [apply updateSmap_uniq; auto | auto].
+Qed.
+
+Lemma se_cmd_dom_mono : forall smap0 sm0 sf0 se0 c,
+  dom smap0 [<=] dom (STerms (se_cmd (mkSstate smap0 sm0 sf0 se0) c)).
+Proof.
+  intros smap0 sm0 sf0 se0 c.
+  assert (forall sm id0 st0, dom sm [<=] dom (updateSmap sm id0 st0)) as J.
+    intros. assert (J:=@updateSmap_dom_eq sm id0 st0). fsetdec. 
+  destruct c; simpl; try solve [eauto using J| fsetdec].
+Qed.
+
+Lemma lookupSmap_in : forall sm id0 st0,
+  uniq sm ->
+  binds id0 st0 sm ->
+  lookupSmap sm id0 = st0.
+Proof.
+  induction sm; intros.
+    inversion H0.
+
+    destruct a.
+    simpl in *.
+    inversion H; subst.
+    destruct (@eq_dec atom (@EqDec_eq_of_EqDec atom EqDec_atom) a id0); subst; simpl;
+      analyze_binds_uniq H0; auto.
+Qed.
+
+Lemma id2Sterm_in : forall sm id0 st0,
+  uniq sm ->
+  binds id0 st0 sm ->
+  value2Sterm sm (value_id id0) = st0.
+Proof.
+  intros. simpl. apply lookupSmap_in; auto.
+Qed.
+
+Lemma lookupSmap_notin : forall sm id0,
+  uniq sm ->
+  id0 `notin` dom sm ->
+  lookupSmap sm id0 = sterm_val (value_id id0).
+Proof.
+  induction sm; intros; simpl; auto.
+    destruct a.
+    simpl in *.
+    inversion H; subst.
+    destruct (@eq_dec atom (@EqDec_eq_of_EqDec atom EqDec_atom) a id0); subst; simpl;
+      analyze_binds_uniq H0; auto.
+Qed.
+
+Lemma id2Sterm_notin : forall sm id0,
+  uniq sm ->
+  id0 `notin` dom sm ->
+  value2Sterm sm (value_id id0) = sterm_val (value_id id0).
+Proof.
+  intros. simpl. apply lookupSmap_notin; auto.
+Qed.
+
+Lemma const2Sterm : forall sm c,
+  value2Sterm sm (value_const c) = sterm_val (value_const c).
+Proof.
+  intros. auto.
+Qed.
+       
+Lemma updateSmap_inversion : forall sm id0 st0 id1 st1,
+  uniq sm ->
+  binds id1 st1 (updateSmap sm id0 st0) ->
+  (id0 <> id1 /\ binds id1 st1 sm) \/ (id0 = id1 /\ st0 = st1).
+Proof.
+  induction sm; intros id0 st0 id1 st1 Uniq Binds; simpl in Binds.
+    analyze_binds Binds.
+
+    destruct a.
+    inversion Uniq; subst.
+    destruct (a==id0); subst.
+      analyze_binds Binds.
+      left. split; auto.
+        apply binds_In in BindsTac.
+        fsetdec.
+
+      analyze_binds Binds.
+      apply IHsm in BindsTac; auto.
+        destruct BindsTac; auto.
+          destruct H; auto.
+Qed.
+
+            
+Lemma binds_updateSmap_eq : forall sm id0 st0,
+  binds id0 st0 (updateSmap sm id0 st0).
+Proof.
+  induction sm; intros id0 st0; simpl; auto.
+    destruct a.
+    destruct (a == id0); subst; auto.
+Qed.
+
+Lemma binds_updateSmap_neq : forall sm id0 st0 id1 st1,
+  binds id1 st1 sm ->
+  id0 <> id1 ->
+  binds id1 st1 (updateSmap sm id0 st0).
+Proof.
+  induction sm; intros id0 st0 id1 st1 Hbinds id0_neq_id1; simpl; auto.
+    destruct a.
+    simpl_env in Hbinds.
+    analyze_binds Hbinds.
+      destruct (a == id0); subst; auto.
+        contradict id0_neq_id1; auto.
+
+      destruct (a == id0); subst; auto.
+Qed.
+
+Lemma _se_cmd_uniq : forall c sstate0,
+  uniq (STerms sstate0) ->
+  uniq (STerms (se_cmd sstate0 c)).
+Proof.
+  intros c sstate0 Huniq.
+  destruct c; simpl; try solve [apply updateSmap_uniq; auto | auto].
+Qed.
+
+Lemma _se_cmds_uniq : forall cs sstate0,
+  uniq (STerms sstate0) ->
+  uniq (STerms (se_cmds sstate0 cs)).
+Proof.
+  induction cs; intros; simpl; auto using _se_cmd_uniq.
+Qed.
+
+Lemma se_cmds_uniq : forall cs smap0 sm0 sf0 se0,
+  uniq smap0 ->
+  uniq (STerms (se_cmds (mkSstate smap0 sm0 sf0 se0) cs)).
+Proof.
+  intros.
+  apply _se_cmds_uniq; auto. 
+Qed.
+
+Lemma se_cmds_dom_sub: forall smap0 sm0 sf0 se0 cs,
+  dom smap0 [<=]
+    dom (STerms (se_cmds (mkSstate smap0 sm0 sf0 se0) cs)).
+Admitted.
+
+Lemma se_cmds_rev_cons : forall cs c sstate0,
+  se_cmds sstate0 (cs++c::nil) = se_cmd (se_cmds sstate0 cs) c.
+Proof.
+  induction cs; intros; simpl; auto.
+Qed.
+
+Lemma se_cmds_app : forall cs cs' sstate0,
+  se_cmds sstate0 (cs++cs') = se_cmds (se_cmds sstate0 cs) cs'.
+Proof.
+  induction cs; intros; simpl; auto.
+Qed.
+
+Lemma se_cmds_cons : forall cs c sstate0,
+  se_cmds sstate0 ((c::nil)++cs) = se_cmds (se_cmd sstate0 c) cs.
+Proof.
+  induction cs; intros; simpl; auto.
+Qed.
+
+
+(***************************************************************)
+(* Denotational semantics of symbolic exe *)
+
+Inductive sterm_denotes_genericvalue : 
+   layouts ->               (* CurTatgetData *)
+   GVMap ->                 (* local registers *)
+   GVMap ->                 (* global variables *)
+   mem ->                   (* Memory *)
+   sterm ->                 (* symbolic term *)
+   GenericValue ->          (* value that denotes sterm *)
+   Prop :=
+| sterm_val_denotes : forall TD lc gl Mem v gv,
+  getOperandValue TD v lc gl = Some gv ->  
+  sterm_denotes_genericvalue TD lc gl Mem (sterm_val v) gv
+| sterm_bop_denotes : forall TD lc gl Mem op0 sz0 st1 st2 gv1 gv2 gv3,
+  sterm_denotes_genericvalue TD lc gl Mem st1 gv1 ->
+  sterm_denotes_genericvalue TD lc gl Mem st2 gv2 ->
+  mbop TD op0 sz0 gv1 gv2 = Some gv3 ->
+  sterm_denotes_genericvalue TD lc gl Mem (sterm_bop op0 sz0 st1 st2) gv3
+| sterm_extractvalue_denotes : forall TD lc gl Mem t1 st1 idxs0 gv1 gv2,
+  sterm_denotes_genericvalue TD lc gl Mem st1 gv1 ->
+  extractGenericValue TD t1 gv1 idxs0 = Some gv2 ->
+  sterm_denotes_genericvalue TD lc gl Mem (sterm_extractvalue t1 st1 idxs0) gv2
+| sterm_insertvalue_denotes : forall TD lc gl Mem t1 st1 t2 st2 idxs0 gv1 gv2 gv3,
+  sterm_denotes_genericvalue TD lc gl Mem st1 gv1 ->
+  sterm_denotes_genericvalue TD lc gl Mem st2 gv2 ->
+  insertGenericValue TD t1 gv1 idxs0 t2 gv2 = Some gv3 ->
+  sterm_denotes_genericvalue TD lc gl Mem (sterm_insertvalue t1 st1 t2 st2 idxs0) gv3
+| sterm_malloc_denotes : forall TD lc gl Mem0 Mem1 sm0 t0 sz0 align0 tsz0 Mem2 mb,
+  smem_denotes_mem TD lc gl Mem0 sm0 Mem1 ->
+  getTypeAllocSize TD t0 = Some tsz0 ->
+  malloc TD Mem1 (tsz0 * sz0) align0 = Some (Mem2, mb) ->
+  sterm_denotes_genericvalue TD lc gl Mem0 (sterm_malloc sm0 t0 sz0 align0) (ptr2GV TD (mb, 0))
+| sterm_alloca_denotes : forall TD lc gl Mem0 Mem1 sm0 t0 sz0 align0 tsz0 Mem2 mb,
+  smem_denotes_mem TD lc gl Mem0 sm0 Mem1 ->
+  getTypeAllocSize TD t0 = Some tsz0 ->
+  malloc TD Mem1 (tsz0 * sz0) align0 = Some (Mem2, mb) ->
+  sterm_denotes_genericvalue TD lc gl Mem0 (sterm_alloca sm0 t0 sz0 align0) (ptr2GV TD (mb, 0))
+| sterm_load_denotes : forall TD lc gl Mem0 Mem1 sm0 t0 st0 gv0 mp0 gv1,
+  sterm_denotes_genericvalue TD lc gl Mem0 st0 gv0 ->
+  smem_denotes_mem TD lc gl Mem0 sm0 Mem1 ->
+  GV2ptr TD (getPointerSize TD) gv0 = Some mp0 ->
+  mload TD Mem1 mp0 t0 = Some gv1 ->
+  sterm_denotes_genericvalue TD lc gl Mem0 (sterm_load sm0 t0 st0) gv1
+| sterm_gep_denotes : forall TD lc gl Mem ib0 t0 st0 sts0 gv0 gvs0 ns0 mp0 mp1,
+  sterm_denotes_genericvalue TD lc gl Mem st0 gv0 ->
+  sterms_denote_genericvalues TD lc gl Mem sts0 gvs0 ->
+  GV2ptr TD (getPointerSize TD) gv0 = Some mp0 ->
+  GVs2Nats TD gvs0 = Some ns0 ->
+  mgep TD t0 mp0 ns0 = Some mp1 ->
+  sterm_denotes_genericvalue TD lc gl Mem (sterm_gep ib0 t0 st0 sts0) (ptr2GV TD mp1)
+| sterm_ext_denotes : forall TD lc gl Mem op0 t1 st1 t2 gv1 gv2,
+  sterm_denotes_genericvalue TD lc gl Mem st1 gv1 ->
+  mext TD op0 t1 gv1 t2 = Some gv2 ->
+  sterm_denotes_genericvalue TD lc gl Mem (sterm_ext op0 t1 st1 t2) gv2
+| sterm_cast_denotes : forall TD lc gl Mem op0 t1 st1 t2 gv1 gv2,
+  sterm_denotes_genericvalue TD lc gl Mem st1 gv1 ->
+  mcast TD op0 t1 gv1 t2 = Some gv2 ->
+  sterm_denotes_genericvalue TD lc gl Mem (sterm_cast op0 t1 st1 t2) gv2
+| sterm_icmp_denotes : forall TD lc gl Mem cond0 t0 st1 st2 gv1 gv2 gv3,
+  sterm_denotes_genericvalue TD lc gl Mem st1 gv1 ->
+  sterm_denotes_genericvalue TD lc gl Mem st2 gv2 ->
+  micmp TD cond0 t0 gv1 gv2 = Some gv3 ->
+  sterm_denotes_genericvalue TD lc gl Mem (sterm_icmp cond0 t0 st1 st2) gv3
+| sterm_select_denotes : forall TD lc gl Mem st0 t0 st1 st2 gv0 gv1 gv2 c0 gv3,
+  sterm_denotes_genericvalue TD lc gl Mem st0 gv0 ->
+  sterm_denotes_genericvalue TD lc gl Mem st1 gv1 ->
+  sterm_denotes_genericvalue TD lc gl Mem st2 gv2 ->
+  GV2nat TD 1 gv0 = Some c0 ->
+  (if c0 then gv1 else gv2) = gv3 -> 
+  sterm_denotes_genericvalue TD lc gl Mem (sterm_select st0 t0 st1 st2) gv3
+with sterms_denote_genericvalues : 
+   layouts ->               (* CurTatgetData *)
+   GVMap ->                 (* local registers *)
+   GVMap ->                 (* global variables *)
+   mem ->                   (* Memory *)
+   list sterm ->            (* symbolic terms *)
+   list GenericValue ->     (* values that denote sterms *)
+   Prop :=
+| sterms_nil_denote : forall TD lc gl Mem,
+  sterms_denote_genericvalues TD lc gl Mem nil nil
+| sterms_cons_denote : forall TD lc gl Mem sts st gvs gv,
+  sterms_denote_genericvalues TD lc gl Mem sts gvs ->
+  sterm_denotes_genericvalue TD lc gl Mem st gv ->
+  sterms_denote_genericvalues TD lc gl Mem (st::sts) (gv::gvs)
+with smem_denotes_mem : 
+   layouts ->               (* CurTatgetData *)
+   GVMap ->                 (* local registers *)
+   GVMap ->                 (* global variables *)
+   mem ->                   (* Memory *)
+   smem ->                  (* symbolic mem *)
+   mem ->                   (* value that denotes smem *)
+   Prop :=
+| smem_init_denotes : forall TD lc gl Mem,
+  smem_denotes_mem TD lc gl Mem smem_init Mem
+| smem_malloc_denotes : forall TD lc gl Mem0 Mem1 sm0 t0 sz0 align0 tsz0 Mem2 mb,
+  smem_denotes_mem TD lc gl Mem0 sm0 Mem1 ->
+  getTypeAllocSize TD t0 = Some tsz0 ->
+  malloc TD Mem1 (tsz0 * sz0) align0 = Some (Mem2, mb) ->
+  smem_denotes_mem TD lc gl Mem0 (smem_malloc sm0 t0 sz0 align0) Mem2
+| smem_free_denotes : forall TD lc gl Mem0 Mem1 sm0 t0 st0 gv0 mptr0 Mem2,
+  sterm_denotes_genericvalue TD lc gl Mem0 st0 gv0 ->
+  smem_denotes_mem TD lc gl Mem0 sm0 Mem1 ->
+  GV2ptr TD (getPointerSize TD) gv0 = Some mptr0 ->
+  free Mem1 mptr0 = Some Mem2->
+  smem_denotes_mem TD lc gl Mem0 (smem_free sm0 t0 st0) Mem2
+| smem_alloca_denotes : forall TD lc gl Mem0 Mem1 sm0 t0 sz0 align0 tsz0 Mem2 mb,
+  smem_denotes_mem TD lc gl Mem0 sm0 Mem1 ->
+  getTypeAllocSize TD t0 = Some tsz0 ->
+  malloc TD Mem1 (tsz0 * sz0) align0 = Some (Mem2, mb) ->
+  smem_denotes_mem TD lc gl Mem0 (smem_alloca sm0 t0 sz0 align0) Mem2
+| smem_load_denotes : forall TD lc gl Mem0 sm0 t0 st0 Mem1,
+  smem_denotes_mem TD lc gl Mem0 sm0 Mem1 ->
+  smem_denotes_mem TD lc gl Mem0 (smem_load sm0 t0 st0) Mem1
+| smem_store_denotes : forall TD lc gl Mem0 Mem1 sm0 t0 st1 st2 gv1 gv2 mptr2 Mem2,
+  sterm_denotes_genericvalue TD lc gl Mem0 st1 gv1 ->
+  sterm_denotes_genericvalue TD lc gl Mem0 st2 gv2 ->
+  smem_denotes_mem TD lc gl Mem0 sm0 Mem1 ->
+  GV2ptr TD (getPointerSize TD) gv2 = Some mptr2 ->
+  mstore TD Mem1 mptr2 t0 gv1 = Some Mem2 ->
+  smem_denotes_mem TD lc gl Mem0 (smem_store sm0 t0 st1 st2) Mem2
+.
+
+Inductive sframe_denotes_frame : 
+   layouts ->               (* CurTatgetData *)
+   GVMap ->                 (* local registers *)
+   GVMap ->                 (* global variables *)
+   list mblock ->           (* Track memory allocated by alloca *)
+   mem ->                  (* mem *)
+   sframe ->                (* symbolic frame *)
+   list mblock ->           (* allocas that denotes sframe *)
+   Prop :=
+| sframe_init_denotes : forall TD lc gl Mem als,
+  sframe_denotes_frame TD lc gl als Mem sframe_init als
+| sframe_alloca_denotes : forall TD lc gl Mem0 Mem1 als0 als1 t0 sz0 align0 tsz0 Mem2 mb sm0 sf0,
+  smem_denotes_mem TD lc gl Mem0 sm0 Mem1 ->
+  sframe_denotes_frame TD lc gl als0 Mem0 sf0 als1 ->
+  getTypeAllocSize TD t0 = Some tsz0 ->
+  malloc TD Mem1 (tsz0 * sz0) align0 = Some (Mem2, mb) ->
+  sframe_denotes_frame TD lc gl als0 Mem0 (sframe_alloca sm0 sf0 t0 sz0 align0) (mb::als1)
+.
+
+Inductive seffects_denote_trace : 
+   list sterm ->            (* symbolic effects *)
+   trace ->                 (* trace that denotes seffects *)
+   Prop :=
+| seffects_nil_denote : 
+  seffects_denote_trace nil trace_nil
+.
+
+Hint Constructors sterm_denotes_genericvalue sterms_denote_genericvalues 
+                  smem_denotes_mem sframe_denotes_frame seffects_denote_trace.
+
+Scheme sterm_denotes_genericvalue_ind2 := Induction for sterm_denotes_genericvalue Sort Prop
+  with sterms_denote_genericvalues_ind2 := Induction for sterms_denote_genericvalues Sort Prop
+  with smem_denotes_mem_ind2 := Induction for smem_denotes_mem Sort Prop.
+
+Combined Scheme sd_mutind from sterm_denotes_genericvalue_ind2, 
+                               sterms_denote_genericvalues_ind2, 
+                               smem_denotes_mem_ind2.
+
+Tactic Notation "sd_mutind_cases" tactic(first) tactic(c) :=
+  first;
+[ c "sterm_val_denotes"
+| c "sterm_bop_denotes"
+| c "sterm_extractvalue_denotes"
+| c "sterm_insertvalue_denotes"
+| c "sterm_malloc_denotes"
+| c "sterm_alloca_denotes"
+| c "sterm_load_denotes"
+| c "sterm_gep_denotes"
+| c "sterm_ext_denotes"
+| c "sterm_cast_denotes"
+| c "sterm_icmp_denotes" 
+| c "sterm_select_denotes"
+| c "sterms_nil_denote"
+| c "sterms_cons_denote"
+| c "smem_init_denotes"
+| c "smem_malloc_denotes"
+| c "smem_free_denotes"
+| c "smem_alloca_denotes"
+| c "smem_load_denotes"
+| c "smem_store_denotes" ].
+
+Definition smap_denotes_gvmap TD lc gl Mem smap' lc' gl' :=
+(forall id' st',  
+  binds id' st' smap' ->
+  exists gv',
+    sterm_denotes_genericvalue TD lc gl Mem st' gv' /\
+    lookupEnv id' lc' gl' = Some gv') /\
+(forall id' gv',  
+  lookupEnv id' lc' gl' = Some gv' ->
+  exists st',
+    binds id' st' smap' /\
+    sterm_denotes_genericvalue TD lc gl Mem st' gv'
+).
+
+Definition sstate_denotes_state TD lc gl als Mem sstate' lc' gl' als' mem' tr :=
+smap_denotes_gvmap TD lc gl Mem sstate'.(STerms) lc' gl' /\
+smem_denotes_mem TD lc gl Mem sstate'.(SMem) mem' /\
+sframe_denotes_frame TD lc gl als Mem sstate'.(SFrame) als' /\
+seffects_denote_trace sstate'.(SEffects) tr.
+
+(* Initial smap of a symbolic exe w.r.t a concrete a state. *)
+
+Fixpoint globals_to_smap (gl:GVMap) : smap :=
+match gl with
+| nil => nil
+| (id0, _)::gl' => updateSmap (globals_to_smap gl') id0 (sterm_val (value_id id0)) 
+end.
+
+Fixpoint locals_to_smap (lc:GVMap) (m0:smap) : smap :=
+match lc with
+| nil => m0
+| (id0, _)::lc' => updateSmap (locals_to_smap lc' m0) id0 (sterm_val (value_id id0)) 
+end.
+
+Definition env_to_smap (gl lc:GVMap) : smap :=
+locals_to_smap lc (globals_to_smap gl).
+
+Lemma globals_to_smap_dom_eq : forall gl,
+  dom (globals_to_smap gl) [=] dom gl.
+Proof.
+  induction gl; simpl.
+    fsetdec.
+
+    destruct a.
+    rewrite <- IHgl. clear IHgl.
+    rewrite updateSmap_dom_eq. fsetdec.
+Qed.
+
+Lemma locals_to_smap_dom_eq : forall lc m0,
+  dom (locals_to_smap lc m0) [=] dom lc `union` dom m0.
+Proof.
+  induction lc; intros m0; simpl.
+    fsetdec.
+
+    destruct a.
+    rewrite updateSmap_dom_eq. 
+    rewrite IHlc.
+    fsetdec.
+Qed.
+
+Lemma env_to_smap_dom_eq : forall gl lc,
+  dom (env_to_smap gl lc) [=] dom gl `union` dom lc.
+Proof.
+  intros gl lc.
+  unfold env_to_smap.
+  rewrite locals_to_smap_dom_eq.
+  rewrite globals_to_smap_dom_eq.
+  fsetdec.
+Qed.
+
+Lemma globals_to_smap_uniq : forall gl,
+  uniq (globals_to_smap gl).
+Proof.
+  induction gl; simpl; auto.
+    destruct a.
+    apply updateSmap_uniq; auto.
+Qed.
+
+Lemma locals_to_smap_uniq : forall lc m0,
+  uniq m0 ->
+  uniq (locals_to_smap lc m0).
+Proof.
+  induction lc; simpl; intros; auto.
+    destruct a.
+    apply updateSmap_uniq; auto.
+Qed.
+
+Lemma env_to_smap_uniq : forall gl lc,
+  uniq (env_to_smap gl lc).
+Proof.
+  intros gl lc.
+  unfold env_to_smap.
+  apply locals_to_smap_uniq.
+  apply globals_to_smap_uniq.
+Qed.
+
+Lemma binds_globals_to_smap : forall gl id0 st0,
+  uniq gl ->
+  binds id0 st0 (globals_to_smap gl) ->
+  st0 = sterm_val (value_id id0) /\ 
+  exists gv, lookupGVMap gl id0 = Some gv.
+Proof.
+  induction gl; intros; simpl in *.
+    inversion H0.
+
+    inversion H; subst.
+    apply updateSmap_inversion in H0; auto using globals_to_smap_uniq.
+    destruct (@eq_dec id (@EqDec_eq_of_EqDec id EqDec_atom) id0 x); subst; simpl; auto.
+      destruct H0 as [[J1 J2] | [J1 J2]].
+        contradict J1; auto.
+        split; auto. exists a0. auto.
+     
+      destruct H0 as [[J1 J2] | [J1 J2]].
+        apply IHgl in J2; auto.
+
+        contradict n; auto.
+Qed.
+
+Lemma binds_locals_to_smap : forall id0 st0 lc m0,
+  uniq m0 ->
+  uniq lc ->
+  binds id0 st0 (locals_to_smap lc m0) ->
+  (st0 = sterm_val (value_id id0) /\ exists gv, lookupGVMap lc id0 = Some gv) \/
+  binds id0 st0 m0.  
+Proof.
+  induction lc; intros; simpl in *; auto.
+    inversion H0; subst.
+    apply updateSmap_inversion in H1; auto using locals_to_smap_uniq.
+    destruct (@eq_dec id (@EqDec_eq_of_EqDec id EqDec_atom) id0 x); subst; simpl; auto.
+      destruct H1 as [[J1 J2] | [J1 J2]].
+        contradict J1; auto.
+        left. split; auto. exists a0. auto.
+     
+      destruct H1 as [[J1 J2] | [J1 J2]].
+        apply IHlc in J2; auto.
+
+        contradict n; auto.
+Qed.
+
+Lemma binds_env_to_smap : forall TD id0 st0 gl lc,
+  uniq gl ->
+  uniq lc -> 
+  binds id0 st0 (env_to_smap gl lc) ->
+  st0 = sterm_val (value_id id0) /\ 
+  exists gv, getOperandValue TD (value_id id0) lc gl = Some gv.
+Proof.
+  intros.
+  apply binds_locals_to_smap in H1; auto using globals_to_smap_uniq.
+  destruct H1 as [[J1 [gv J2]] | H1]; subst.
+    split; auto. simpl. unfold lookupEnv. rewrite J2. exists gv. auto.
+    apply binds_globals_to_smap in H1; auto using globals_to_smap_uniq.
+    destruct H1 as [J1 [gv J2]]; auto.
+      split; auto. simpl. unfold lookupEnv. rewrite J2. 
+      destruct (lookupGVMap lc id0).
+        exists g. auto.
+        exists gv. auto.
+Qed.
+
+Lemma env_to_smap_denotes__imples__gv : forall id0 st0 TD Mem0 gl lc,
+  uniq gl ->
+  uniq lc -> 
+  binds id0 st0 (env_to_smap gl lc) ->
+  exists gv0,
+    sterm_denotes_genericvalue TD lc gl Mem0 st0 gv0 /\
+    lookupEnv id0 lc gl = Some gv0.
+Proof.
+  intros id0 st0 TD Mem0 gl lc Uniqg Uniqc Binds.
+  apply binds_env_to_smap with (TD:=TD) in Binds; auto.
+  destruct Binds as [J1 [gv0 J2]]; subst.
+  exists gv0. split; auto.
+Qed.
+
+Lemma lookupEnv_globals_to_smap : forall gl id0 gv0,
+  lookupGVMap gl id0 = Some gv0 ->
+  binds id0 (sterm_val (value_id id0)) (globals_to_smap gl).
+Proof.
+  induction gl; intros; simpl in *.
+    inversion H.
+    destruct a.
+    destruct (id0==i0); subst.
+      inversion H; subst. 
+      apply binds_updateSmap_eq; auto.
+
+      apply binds_updateSmap_neq; eauto.
+Qed.
+
+Lemma lookupEnv_locals_to_smap : forall lc m1 id0 gv0,
+  lookupGVMap lc id0 = Some gv0 ->
+  binds id0 (sterm_val (value_id id0)) (locals_to_smap lc m1).
+Proof.
+  induction lc; intros; simpl in *.
+    inversion H.
+    destruct a.
+    destruct (id0==i0); subst.
+      inversion H; subst. 
+      apply binds_updateSmap_eq; auto.
+
+      apply binds_updateSmap_neq; eauto.
+Qed.
+
+Lemma lookupEnv_locals_to_smap' : forall lc m1 st0 id0,
+  lookupGVMap lc id0 = None ->
+  binds id0 st0 m1 ->
+  binds id0 st0 (locals_to_smap lc m1).
+Proof.
+  induction lc; intros; simpl in *; auto.
+    destruct a.
+    destruct (id0==i0); subst.
+      inversion H.    
+      apply binds_updateSmap_neq; eauto.
+Qed.
+
+Lemma lookupEnv_env_to_smap : forall id0 gv0 gl lc,
+  lookupEnv id0 lc gl = Some gv0 ->
+  binds id0 (sterm_val (value_id id0)) (env_to_smap gl lc).
+Proof.
+  intros.
+  unfold lookupEnv in H.
+  unfold env_to_smap.
+  remember (lookupGVMap lc id0) as ogv.
+  destruct ogv.
+    inversion H; subst.
+    eapply lookupEnv_locals_to_smap; eauto.
+
+    apply lookupEnv_locals_to_smap'; auto.
+    apply lookupEnv_globals_to_smap in H; auto.
+Qed.
+
+Lemma gv__imples__env_to_smap_denotes : forall id0 TD Mem0 gl lc gv0,
+  lookupEnv id0 lc gl = Some gv0 ->
+  binds id0 (sterm_val (value_id id0)) (env_to_smap gl lc) /\
+  sterm_denotes_genericvalue TD lc gl Mem0 (sterm_val (value_id id0)) gv0.
+Proof.
+  intros id0 TD Mem0 gl lc gv0 Binds.
+  split.
+    eapply lookupEnv_env_to_smap; eauto.
+
+    apply sterm_val_denotes; auto.
+Qed.
+
+Lemma env_to_smap_denotes_gvmap :forall TD lc gl Mem0,
+  uniq gl ->
+  uniq lc ->
+  smap_denotes_gvmap TD lc gl Mem0 (env_to_smap gl lc) lc gl.
+Proof.
+  intros TD lc gl Mem0 Uniqg Uniqc.
+  unfold smap_denotes_gvmap.
+  split; intros.
+    apply env_to_smap_denotes__imples__gv; auto.
+
+    exists (sterm_val (value_id id')).
+    apply gv__imples__env_to_smap_denotes; auto.
+Qed.
+
+Lemma env_to_smap_denotes_id :forall TD lc gl als Mem0,
+  uniq gl ->
+  uniq lc ->
+  sstate_denotes_state TD lc gl als Mem0 (mkSstate (env_to_smap gl lc) smem_init sframe_init nil) lc gl als Mem0 trace_nil.
+Proof.
+  intros TD lc gl als Mem0 Uniqg Uniqc.
+  split; simpl; auto using env_to_smap_denotes_gvmap.
+Qed.
+
+Lemma se_cmds_env_to_smap_dom_sub: forall lc0 gl0 cs,
+  union (dom lc0) (dom gl0) [<=]
+    dom (STerms (se_cmds (mkSstate (env_to_smap gl0 lc0) smem_init sframe_init nil) cs)).
+Admitted.
+
+(* The denotational rules are determinastic. *)
+
+Definition sterm_denotes_genericvalue_det_prop TD lc gl Mem0 st0 gv1 
+  (sd:sterm_denotes_genericvalue TD lc gl Mem0 st0 gv1) :=
+  forall gv2,
+  sterm_denotes_genericvalue TD lc gl Mem0 st0 gv2 ->
+  gv1 = gv2.
+
+Definition sterms_denote_genericvalues_det_prop TD lc gl Mem0 sts0 gvs1
+  (ds:sterms_denote_genericvalues TD lc gl Mem0 sts0 gvs1) :=
+  forall gvs2,
+  sterms_denote_genericvalues TD lc gl Mem0 sts0 gvs2 ->
+  gvs1 = gvs2.
+
+Definition smem_denotes_mem_det_prop TD lc gl Mem0 st0 Mem1
+  (sd:smem_denotes_mem TD lc gl Mem0 st0 Mem1) :=
+  forall Mem2,
+  smem_denotes_mem TD lc gl Mem0 st0 Mem2 ->
+  Mem1 = Mem2.
+
+Lemma sdenotes_det : 
+  (forall TD lc gl Mem0 st0 gv1 sd, @sterm_denotes_genericvalue_det_prop TD lc gl Mem0 st0 gv1 sd) /\
+  (forall TD lc gl Mem0 sts0 gvs1 sd, @sterms_denote_genericvalues_det_prop TD lc gl Mem0 sts0 gvs1 sd) /\
+  (forall TD lc gl Mem0 st0 Mem1 sd, @smem_denotes_mem_det_prop TD lc gl Mem0 st0 Mem1 sd).
+Proof.
+(sd_mutind_cases
+  apply sd_mutind with
+    (P  := sterm_denotes_genericvalue_det_prop)
+    (P0 := sterms_denote_genericvalues_det_prop)
+    (P1 := smem_denotes_mem_det_prop) Case);
+  unfold sterm_denotes_genericvalue_det_prop, 
+         sterms_denote_genericvalues_det_prop, 
+         smem_denotes_mem_det_prop; intros.
+Case "sterm_val_denotes".
+  inversion H; subst.
+  rewrite e in H5. inversion H5; auto.
+Case "sterm_bop_denotes".
+  inversion H1; subst.
+  apply H in H11; subst.
+  apply H0 in H12; subst.
+  rewrite H13 in e.
+  inversion e; auto.
+Case "sterm_extractvalue_denotes".
+  inversion H0; subst.
+  apply H in H9; subst.
+  rewrite H10 in e.
+  inversion e; auto.
+Case "sterm_insertvalue_denotes".
+  inversion H1; subst.
+  apply H in H12; subst.
+  apply H0 in H13; subst.
+  rewrite H14 in e.
+  inversion e; auto.
+Case "sterm_malloc_denotes".
+  inversion H0; subst.
+  rewrite e in H11. inversion H11; subst.
+  apply H in H10; subst.
+  rewrite H12 in e0. inversion e0; auto.
+Case "sterm_alloca_denotes".
+  inversion H0; subst.
+  rewrite e in H11. inversion H11; subst.
+  apply H in H10; subst.
+  rewrite H12 in e0. inversion e0; auto.
+Case "sterm_load_denotes".
+  inversion H1; subst.
+  apply H0 in H10; subst.
+  apply H in H5; subst.
+  rewrite e in H12. inversion H12; subst.
+  rewrite H13 in e0. inversion e0; auto.
+Case "sterm_gep_denotes".
+  inversion H1; subst.
+  apply H in H6; subst.
+  apply H0 in H11; subst.
+  rewrite H13 in e. inversion e; subst.
+  rewrite H14 in e0. inversion e0; subst.
+  rewrite H15 in e1. inversion e1; auto.
+Case "sterm_ext_denotes".
+  inversion H0; subst.
+  apply H in H10; subst.
+  rewrite H11 in e.
+  inversion e; auto.
+Case "sterm_cast_denotes".
+  inversion H0; subst.
+  apply H in H10; subst.
+  rewrite H11 in e.
+  inversion e; auto.
+Case "sterm_icmp_denotes".
+  inversion H1; subst.
+  apply H in H11; subst.
+  apply H0 in H12; subst.
+  rewrite H13 in e. inversion e; auto.
+Case "sterm_select_denotes".
+  inversion H2; subst.
+  apply H in H7; subst.
+  apply H0 in H12; subst.
+  apply H1 in H14; subst.
+  rewrite H15 in e. inversion e; auto.
+Case "sterms_nil_denote".
+  inversion H; auto.
+Case "sterms_cons_denote".
+  inversion H1; subst.
+  apply H in H8; subst.
+  apply H0 in H10; subst; auto.
+Case "smem_init_denotes".
+  inversion H; auto.
+Case "smem_malloc_denotes".
+  inversion H0; subst.
+  apply H in H10; subst. 
+  rewrite H11 in e. inversion e; subst.
+  rewrite H12 in e0. inversion e0; auto.
+Case "smem_free_denotes".
+  inversion H1; subst.
+  apply H in H5; subst. 
+  apply H0 in H10; subst. 
+  rewrite H12 in e. inversion e; subst.
+  rewrite H13 in e0. inversion e0; auto.
+Case "smem_alloca_denotes".
+  inversion H0; subst.
+  apply H in H10; subst. 
+  rewrite H11 in e. inversion e; subst.
+  rewrite H12 in e0. inversion e0; auto.
+Case "smem_load_denotes".
+  inversion H0; subst.
+  apply H in H9; auto. 
+Case "smem_store_denotes".
+  inversion H2; subst.
+  apply H in H7; subst. 
+  apply H0 in H12; subst. 
+  apply H1 in H14; subst. 
+  rewrite H15 in e. inversion e; subst.
+  rewrite H16 in e0. inversion e0; auto.
+Qed.
+
+Lemma sterm_denotes_genericvalue_det : forall TD lc gl Mem0 st0 gv1 gv2,
+  sterm_denotes_genericvalue TD lc gl Mem0 st0 gv1 ->
+  sterm_denotes_genericvalue TD lc gl Mem0 st0 gv2 ->
+  gv1 = gv2.
+Proof.
+  destruct sdenotes_det as [J _].
+  unfold sterm_denotes_genericvalue_det_prop in J.
+  eauto.
+Qed.
+
+Lemma sterms_denote_genericvalues_det : forall TD lc gl Mem0 sts0 gvs1 gvs2,
+  sterms_denote_genericvalues TD lc gl Mem0 sts0 gvs1 ->
+  sterms_denote_genericvalues TD lc gl Mem0 sts0 gvs2 ->
+  gvs1 = gvs2.
+Proof.
+  destruct sdenotes_det as [_ [J _]].
+  unfold sterms_denote_genericvalues_det_prop in J.
+  eauto.
+Qed.
+
+Lemma smem_denotes_mem_det : forall TD lc gl Mem0 st0 Mem1 Mem2,
+  smem_denotes_mem TD lc gl Mem0 st0 Mem1 ->
+  smem_denotes_mem TD lc gl Mem0 st0 Mem2 ->
+  Mem1 = Mem2.
+Proof.
+  destruct sdenotes_det as [_ [_ J]].
+  unfold smem_denotes_mem_det_prop in J.
+  eauto.
+Qed.
+
+Lemma sframe_denotes_frame_det : forall TD lc gl als Mem0 st0 als1 als2,
+  sframe_denotes_frame TD lc gl als Mem0 st0 als1 ->
+  sframe_denotes_frame TD lc gl als Mem0 st0 als2 ->
+  als1 = als2.
+Proof.
+  intros.
+  generalize dependent als2.
+  induction H; intros.
+    inversion H0; auto.
+
+    inversion H3; subst.
+    apply smem_denotes_mem_det with (Mem1:=Mem4) in H; auto; subst.
+    rewrite H1 in H17. inversion H17; subst.
+    rewrite H18 in H2. inversion H2; subst.
+    apply IHsframe_denotes_frame in H16; subst; auto.
+Qed.
+
+Lemma seffects_denote_trace_det : forall ses tr1 tr2,
+  seffects_denote_trace ses tr1 ->
+  seffects_denote_trace ses tr2 ->
+  tr1 = tr2.
+Proof.
+  intros. 
+  inversion H; subst.
+  inversion H0; subst; auto.
+Qed.
+
+Lemma smap_denotes_gvmap_det : forall TD lc gl Mem0 smap0 lc1 gl1 lc2 gl2,
+  smap_denotes_gvmap TD lc gl Mem0 smap0 lc1 gl1 ->
+  smap_denotes_gvmap TD lc gl Mem0 smap0 lc2 gl2 ->
+  eqEnv lc1 gl1 lc2 gl2.
+Proof.
+  intros TD lc gl Mem0 smap0 lc1 gl1 lc2 gl2 J1 J2.
+  destruct J1 as [J11 J12].
+  destruct J2 as [J21 J22].
+  intros id0.
+  remember (lookupEnv id0 lc1 gl1) as ogv1.
+  remember (lookupEnv id0 lc2 gl2) as ogv2.
+  destruct ogv1 as [gv1 | ].
+    symmetry in Heqogv1.
+    apply J12 in Heqogv1.
+    destruct Heqogv1 as [st0 [binds_id0_st0 st0_denotes_gv1]].
+    apply J21 in binds_id0_st0.
+    destruct binds_id0_st0 as [gv' [st0_denotes_gv' id0_gv'_in_env2]].
+    rewrite id0_gv'_in_env2 in Heqogv2.
+    apply sterm_denotes_genericvalue_det with (gv2:=gv1) in st0_denotes_gv'; auto.
+    subst. auto.
+    
+  destruct ogv2 as [gv2 | ]; auto.
+    symmetry in Heqogv2.
+    apply J22 in Heqogv2.
+    destruct Heqogv2 as [st0 [binds_id0_st0 st0_denotes_gv2]].
+    apply J11 in binds_id0_st0.
+    destruct binds_id0_st0 as [gv' [st0_denotes_gv' id0_gv'_in_env1]].
+    rewrite id0_gv'_in_env1 in Heqogv1.
+    inversion Heqogv1.
+Qed.
+
+Lemma sstate_denotes_state_det : forall TD lc gl als Mem0 sstate0 lc1 gl1 als1 Mem1 tr1 lc2 gl2 als2 Mem2 tr2,
+  sstate_denotes_state TD lc gl als Mem0 sstate0 lc1 gl1 als1 Mem1 tr1 ->
+  sstate_denotes_state TD lc gl als Mem0 sstate0 lc2 gl2 als2 Mem2 tr2 ->
+  eqEnv lc1 gl1 lc2 gl2 /\ als1 = als2 /\ Mem1 = Mem2 /\ tr1 = tr2.
+Proof.
+  intros TD lc gl als Mem0 sstate0 lc1 gl1 als1 Mem1 tr1 lc2 gl2 als2 Mem2 tr2 J1 J2.
+  destruct J1 as [J11 [J12 [J13 J14]]].
+  destruct J2 as [J21 [J22 [J23 J24]]].
+  apply smem_denotes_mem_det with (Mem2:=Mem2) in J12; auto; subst.
+  apply sframe_denotes_frame_det with (als2:=als2) in J13; auto; subst.
+  apply seffects_denote_trace_det with (tr2:=tr2) in J14; auto; subst.
+  apply smap_denotes_gvmap_det with (lc2:=lc2)(gl2:=gl2) in J11; auto.
+Qed.
+
+Lemma smap_denotes_gvmap_eqEnv : forall TD lc gl Mem0 smap0 lc1 gl1 lc2 gl2,
+  smap_denotes_gvmap TD lc gl Mem0 smap0 lc1 gl1 ->
+  eqEnv lc1 gl1 lc2 gl2 ->
+  smap_denotes_gvmap TD lc gl Mem0 smap0 lc2 gl2.
+Proof.
+  intros TD lc gl Mem0 smap0 lc1 gl1 lc2 gl2 [H1 H2] H3.
+  split; intros.
+    apply H1 in H.
+    destruct H as [gv' [st'_denotes_gv' id'_gv'_is_env1]].
+    exists gv'. rewrite <- H3.
+    split; auto.
+
+    rewrite <- H3 in H.
+    apply H2 in H; auto.
+Qed.
+
+
+End SimpleSE.
