src/TV/symexe_sound.v
@@ -1,0 +1,1089 @@
+Add LoadPath "../ssa/ott".
+Add LoadPath "../ssa/monads".
+Add LoadPath "../ssa".
+Add LoadPath "../../../theory/metatheory".
+Require Import ssa.
+Require Import List.
+Require Export targetdata.
+Require Import monad.
+Require Import Arith.
+Require Import Metatheory.
+Require Import ssa_mem.
+Require Import genericvalues.
+Require Import ssa_dynamic.
+Require Import trace.
+Require Import symexe_def.
+Require Import symexe_complete.
+
+Export SimpleSE.
+
+(* Symbolic execuction is sound:
+   Given a concrete initial state and that its symbolic execution results
+   denote some concrete states w.r.t the initial state, it is possible to
+   execute the subblock to completion from this initial state. *)
+
+Lemma value2Sterm_denotes__implies__genericvalue : forall TD lc0 gl0 Mem0 smap1 lc gl v gv,
+  uniq smap1 ->
+  (dom lc0 `union` dom gl0) [<=] dom smap1 ->
+  smap_denotes_gvmap TD lc0 gl0 Mem0 smap1 lc gl ->
+  sterm_denotes_genericvalue TD lc0 gl0 Mem0 (value2Sterm smap1 v) gv ->
+  getOperandValue TD v lc gl = Some gv.
+Proof.
+  intros D lc0 gl0 Mem0 smap1 lc gl v gv Huniq Hsub Hdenotes J.
+  unfold smap_denotes_gvmap in Hdenotes.
+  destruct Hdenotes as [J1 J2].
+  destruct v.
+    destruct (@AtomSetProperties.In_dec i0 (dom smap1)) as [i0_in_sstate1 | i0_notin_sstate1].
+      apply binds_In_inv in i0_in_sstate1.
+      destruct i0_in_sstate1 as [st0 Binds].
+      rewrite id2Sterm_in with (st0:=st0) in J; auto.
+      apply J1 with (id':=i0) in Binds.
+      destruct Binds as [gv' [J3 J4]].
+      apply sterm_denotes_genericvalue_det with (gv2:=gv') in J; auto.
+      subst. auto.
+
+      rewrite id2Sterm_notin in J; auto.
+      inversion J; subst.
+      simpl in H4.
+      apply lookupEnv__indom in H4.
+      clear - i0_notin_sstate1 H4 Hsub.
+      contradict H4; fsetdec.
+    rewrite const2Sterm in J.
+    inversion J. auto.
+Qed.
+
+Lemma value2Sterm_denote__imply__genericvalues : forall l0 TD lc0 gl0 Mem0 smap1 lc gl gvs0,
+  uniq smap1 ->
+  (dom lc0 `union` dom gl0) [<=] dom smap1 ->
+  smap_denotes_gvmap TD lc0 gl0 Mem0 smap1 lc gl ->
+  sterms_denote_genericvalues TD lc0 gl0 Mem0 
+    (List.map (value2Sterm smap1) l0) gvs0 ->
+  values2GVs TD l0 lc gl = Some gvs0.
+Proof.
+  induction l0; intros; simpl in *.
+    inversion H2; subst; auto.
+
+    inversion H2; subst.
+    apply value2Sterm_denotes__implies__genericvalue with (lc:=lc)(gl:=gl) in H11; auto.
+    rewrite H11.
+    erewrite IHl0; eauto.
+Qed.
+
+Lemma aux__se_cmd__denotes__exists_op_cmd : forall S TD Ps F B c cs call0 sbs tmn lc arg0 als ECs gl Mem1 lc' gl' als' Mem2 lc0 gl0 als0 Mem0 sstate1 tr1 tr2,
+  uniq sstate1.(STerms) ->
+  (dom lc0 `union` dom gl0) [<=] dom (STerms sstate1) ->
+  sstate_denotes_state TD lc0 gl0 als0 Mem0 sstate1 lc gl als Mem1 tr1 ->
+  sstate_denotes_state TD lc0 gl0 als0 Mem0 (se_cmd sstate1 c) lc' gl' als' Mem2 tr2 ->
+  exists lc', exists gl', exists als', exists Mem2, exists tr,
+    dbCmd (mkState S TD Ps ((mkEC F B ((subblock_intro (c::cs) call0)::sbs) tmn lc arg0 als)::ECs) gl Mem1)
+          (mkState S TD Ps ((mkEC F B ((subblock_intro cs call0)::sbs) tmn lc' arg0 als')::ECs) gl' Mem2) 
+          tr /\
+    tr2 = trace_app tr1 tr.
+Proof.
+  intros S TD Ps F B c cs call0 sbs tmn lc arg0 als ECs gl Mem1 lc' gl' als' Mem2 lc0 gl0 als0 Mem0 sstate1 tr1 tr2 Huniq Hsub Hdenotes1 Hdenotes2.
+  destruct Hdenotes2 as [[Hsterms_denote21 Hsterms_denote22] [Hsmem_denotes2 [Hsframe_denotes2 Hseffects_denote2]]].
+  destruct Hdenotes1 as [Hsterms_denote1 [Hsmem_denotes1 [Hsframe_denotes1 Hseffects_denote1]]].
+  inversion Hseffects_denote1; subst.
+  inversion Hseffects_denote2; subst.
+  (cmd_cases (destruct c) Case).
+  Case "insn_bop".
+    assert (binds i0  
+             (sterm_bop b s (value2Sterm (STerms sstate1) v)
+                            (value2Sterm (STerms sstate1) v0))
+             (STerms (se_cmd sstate1 (insn_bop i0 b s v v0)))) as J.
+      simpl. apply binds_updateSmap_eq; auto.
+    apply Hsterms_denote21 in J.
+    destruct J as [gv3 [bop_denotes_gv3 gv3_in_env']].
+    inversion bop_denotes_gv3; subst.
+    apply value2Sterm_denotes__implies__genericvalue with (lc:=lc)(gl:=gl) in H10; auto.
+    apply value2Sterm_denotes__implies__genericvalue with (lc:=lc)(gl:=gl) in H11; auto.
+    assert (HupdateEnv:=exists_updateEnv lc gl i0 gv3).
+    destruct HupdateEnv as [lc2 [gl2 HupdateEnv]].
+    exists lc2. exists gl2. exists als. exists Mem1. exists trace_nil. 
+    assert (BOP TD lc gl b s v v0 = Some gv3) as J.
+      unfold BOP. rewrite H10. rewrite H11. auto.
+    split; eauto.
+
+  Case "insn_extractvalue".
+    assert (binds i0  
+             (sterm_extractvalue t
+                            (value2Sterm (STerms sstate1) v)
+                            l0)
+             (STerms (se_cmd sstate1 (insn_extractvalue i0 t v l0)))) as J.
+      simpl. apply binds_updateSmap_eq; auto.
+    apply Hsterms_denote21 in J.
+    destruct J as [gv' [extractvalue_denotes_gv' gv_in_env']].
+    inversion extractvalue_denotes_gv'; subst.
+    apply value2Sterm_denotes__implies__genericvalue with (lc:=lc)(gl:=gl) in H9; auto.
+    assert (HupdateEnv:=exists_updateEnv lc gl i0 gv').
+    destruct HupdateEnv as [lc2 [gl2 HupdateEnv]].
+    exists lc2. exists gl2. exists als. exists Mem1. exists trace_nil.
+    split; eauto.
+
+  Case "insn_insertvalue".
+    assert (binds i0  
+             (sterm_insertvalue t
+                            (value2Sterm (STerms sstate1) v)
+                            t0
+                            (value2Sterm (STerms sstate1) v0)
+                            l0)
+             (STerms (se_cmd sstate1 (insn_insertvalue i0 t v t0 v0 l0)))) as J.
+      simpl. apply binds_updateSmap_eq; auto.
+    apply Hsterms_denote21 in J.
+    destruct J as [gv' [insertvalue_denotes_gv' gv_in_env']].
+    inversion insertvalue_denotes_gv'; subst.
+    apply value2Sterm_denotes__implies__genericvalue with (lc:=lc)(gl:=gl) in H11; auto.
+    apply value2Sterm_denotes__implies__genericvalue with (lc:=lc)(gl:=gl) in H12; auto.
+    assert (HupdateEnv:=exists_updateEnv lc gl i0 gv').
+    destruct HupdateEnv as [lc2 [gl2 HupdateEnv]].
+    exists lc2. exists gl2. exists als. exists Mem1. exists trace_nil.
+    split; eauto.
+
+  Case "insn_malloc".
+    assert (binds i0  
+             (sterm_malloc (SMem sstate1) t s a)
+             (STerms (se_cmd sstate1 (insn_malloc i0 t s a)))) as J.
+      simpl. apply binds_updateSmap_eq; auto.
+    apply Hsterms_denote21 in J.
+    destruct J as [gv' [malloc_denotes_gv' gv_in_env']].
+    inversion malloc_denotes_gv'; subst.
+    assert (HupdateEnv:=exists_updateEnv lc gl i0 (ptr2GV TD (mb, 0))).
+    destruct HupdateEnv as [lc2 [gl2 HupdateEnv]].
+    apply smem_denotes_mem_det with (Mem2:=Mem1) in H10; auto.
+    subst.
+    exists lc2. exists gl2. exists als. exists Mem5. exists trace_nil.
+    split; eauto.
+
+  Case "insn_free".
+    inversion Hsmem_denotes2; subst.
+    apply value2Sterm_denotes__implies__genericvalue with (lc:=lc)(gl:=gl) in H4; auto.
+    apply smem_denotes_mem_det with (Mem2:=Mem1) in H9; auto.
+    subst.
+    exists lc. exists gl. exists als. exists Mem2. exists trace_nil.
+    assert (getOperandPtr TD v lc gl = Some mptr0) as J.
+      unfold getOperandPtr. rewrite H4. auto.
+    split; eauto.
+
+  Case "insn_alloca".
+    assert (binds i0  
+             (sterm_alloca (SMem sstate1) t s a)
+             (STerms (se_cmd sstate1 (insn_alloca i0 t s a)))) as J.
+      simpl. apply binds_updateSmap_eq; auto.
+    apply Hsterms_denote21 in J.
+    destruct J as [gv' [alloca_denotes_gv' gv_in_env']].
+    inversion alloca_denotes_gv'; subst.
+    assert (HupdateEnv:=exists_updateEnv lc gl i0 (ptr2GV TD (mb, 0))).
+    destruct HupdateEnv as [lc2 [gl2 HupdateEnv]].
+    apply smem_denotes_mem_det with (Mem2:=Mem1) in H10; auto.
+    subst.
+    exists lc2. exists gl2. exists (mb::als). exists Mem5. exists trace_nil.
+    split; eauto.
+
+  Case "insn_load".
+    assert (binds i0  
+             (sterm_load (SMem sstate1)
+                         t
+                         (value2Sterm (STerms sstate1) v))
+             (STerms (se_cmd sstate1 (insn_load i0 t v)))) as J.
+      simpl. apply binds_updateSmap_eq; auto.
+    apply Hsterms_denote21 in J.
+    destruct J as [gv' [load_denotes_gv' gv_in_env']].
+    inversion load_denotes_gv'; subst.
+    apply value2Sterm_denotes__implies__genericvalue with (lc:=lc)(gl:=gl) in H4; auto.
+    assert (HupdateEnv:=exists_updateEnv lc gl i0 gv').
+    destruct HupdateEnv as [lc2 [gl2 HupdateEnv]].
+    apply smem_denotes_mem_det with (Mem2:=Mem1) in H9; auto.
+    subst.
+    exists lc2. exists gl2. exists als. exists Mem1. exists trace_nil.
+    assert (getOperandPtr TD v lc gl = Some mp0) as J.
+      unfold getOperandPtr. rewrite H4. auto.
+    split; eauto.
+
+  Case "insn_store".
+    inversion Hsmem_denotes2; subst.
+    apply value2Sterm_denotes__implies__genericvalue with (lc:=lc)(gl:=gl) in H5; auto.
+    apply value2Sterm_denotes__implies__genericvalue with (lc:=lc)(gl:=gl) in H10; auto.
+    apply smem_denotes_mem_det with (Mem2:=Mem1) in H12; auto.
+    subst.
+    exists lc. exists gl. exists als. exists Mem2. exists trace_nil.
+    assert (getOperandPtr TD v0 lc gl = Some mptr2) as J.
+      unfold getOperandPtr. rewrite H10. auto.
+    split; eauto.
+
+  Case "insn_gep".
+    assert (binds i0  
+             (sterm_gep i1
+                        t
+                        (value2Sterm (STerms sstate1) v) (List.map (value2Sterm (STerms sstate1)) l0))
+             (STerms (se_cmd sstate1 (insn_gep i0 i1 t v l0)))) as J.
+      simpl. apply binds_updateSmap_eq; auto.
+    apply Hsterms_denote21 in J.
+    destruct J as [gv' [gep_denotes_gv' gv_in_env']].
+    inversion gep_denotes_gv'; subst.
+    apply value2Sterm_denotes__implies__genericvalue with (lc:=lc)(gl:=gl) in H5; auto.
+    apply value2Sterm_denote__imply__genericvalues with (lc:=lc)(gl:=gl) in H10; auto.
+    assert (HupdateEnv:=exists_updateEnv lc gl i0 (ptr2GV TD mp1)).
+    destruct HupdateEnv as [lc2 [gl2 HupdateEnv]].
+    exists lc2. exists gl2. exists als. exists Mem1. exists trace_nil.
+    assert (getOperandPtr TD v lc gl = Some mp0) as J.
+      unfold getOperandPtr. rewrite H5. auto.
+    assert (GEP TD lc gl t mp0 l0 i1 = Some mp1) as J'.
+      unfold GEP.
+      rewrite <- values2GVs_GVs2Nats__intValues2Nats with (gvs0:=gvs0); auto.
+      rewrite H13. auto.
+    split; eauto.
+
+  Case "insn_ext".
+    assert (binds i0  
+             (sterm_ext e t (value2Sterm (STerms sstate1) v) t0)
+             (STerms (se_cmd sstate1 (insn_ext i0 e t v t0)))) as J.
+      simpl. apply binds_updateSmap_eq; auto.
+    apply Hsterms_denote21 in J.
+    destruct J as [gv3 [ext_denotes_gv3 gv3_in_env']].
+    inversion ext_denotes_gv3; subst.
+    apply value2Sterm_denotes__implies__genericvalue with (lc:=lc)(gl:=gl) in H10; auto.
+    assert (HupdateEnv:=exists_updateEnv lc gl i0 gv3).
+    destruct HupdateEnv as [lc2 [gl2 HupdateEnv]].
+    exists lc2. exists gl2. exists als. exists Mem1. exists trace_nil. 
+    assert (EXT TD lc gl e t v t0 = Some gv3) as J.
+      unfold EXT. rewrite H10. auto.
+    split; eauto.
+
+  Case "insn_cast".
+    assert (binds i0  
+             (sterm_cast c t (value2Sterm (STerms sstate1) v) t0)
+             (STerms (se_cmd sstate1 (insn_cast i0 c t v t0)))) as J.
+      simpl. apply binds_updateSmap_eq; auto.
+    apply Hsterms_denote21 in J.
+    destruct J as [gv3 [cast_denotes_gv3 gv3_in_env']].
+    inversion cast_denotes_gv3; subst.
+    apply value2Sterm_denotes__implies__genericvalue with (lc:=lc)(gl:=gl) in H10; auto.
+    assert (HupdateEnv:=exists_updateEnv lc gl i0 gv3).
+    destruct HupdateEnv as [lc2 [gl2 HupdateEnv]].
+    exists lc2. exists gl2. exists als. exists Mem1. exists trace_nil. 
+    assert (CAST TD lc gl c t v t0 = Some gv3) as J.
+      unfold CAST. rewrite H10. auto.
+    split; eauto.
+
+  Case "insn_icmp".
+    assert (binds i0  
+             (sterm_icmp c t (value2Sterm (STerms sstate1) v)
+                             (value2Sterm (STerms sstate1) v0))
+             (STerms (se_cmd sstate1 (insn_icmp i0 c t v v0)))) as J.
+      simpl. apply binds_updateSmap_eq; auto.
+    apply Hsterms_denote21 in J.
+    destruct J as [gv3 [icmp_denotes_gv3 gv3_in_env']].
+    inversion icmp_denotes_gv3; subst.
+    apply value2Sterm_denotes__implies__genericvalue with (lc:=lc)(gl:=gl) in H10; auto.
+    apply value2Sterm_denotes__implies__genericvalue with (lc:=lc)(gl:=gl) in H11; auto.
+    assert (HupdateEnv:=exists_updateEnv lc gl i0 gv3).
+    destruct HupdateEnv as [lc2 [gl2 HupdateEnv]].
+    exists lc2. exists gl2. exists als. exists Mem1. exists trace_nil. 
+    assert (ICMP TD lc gl c t v v0 = Some gv3) as J.
+      unfold ICMP. rewrite H10. rewrite H11. auto.
+    split; eauto.
+
+  Case "insn_select".
+    assert (binds i0  
+             (sterm_select (value2Sterm (STerms sstate1) v)
+                           t
+                           (value2Sterm (STerms sstate1) v0)
+                           (value2Sterm (STerms sstate1) v1))
+             (STerms (se_cmd sstate1 (insn_select i0 v t v0 v1)))) as J.
+      simpl. apply binds_updateSmap_eq; auto.
+    apply Hsterms_denote21 in J.
+    destruct J as [gv3 [select_denotes_gv3 gv3_in_env']].
+    inversion select_denotes_gv3; subst.
+    apply value2Sterm_denotes__implies__genericvalue with (lc:=lc)(gl:=gl) in H5; auto.
+    apply value2Sterm_denotes__implies__genericvalue with (lc:=lc)(gl:=gl) in H10; auto.
+    apply value2Sterm_denotes__implies__genericvalue with (lc:=lc)(gl:=gl) in H12; auto.
+    assert (HupdateEnv:=exists_updateEnv lc gl i0 (if c0 then gv1 else gv2)).
+    destruct HupdateEnv as [lc2 [gl2 HupdateEnv]].
+    exists lc2. exists gl2. exists als. exists Mem1. exists trace_nil. 
+    split; eauto.
+    assert (getOperandInt TD 1 v lc gl = Some c0) as J.
+      unfold getOperandInt. rewrite H5. auto.
+    assert ((lc2, gl2) = if c0 then updateEnv lc gl i0 gv1 else updateEnv lc gl i0 gv2) as J'.
+      destruct c0; auto.
+    eapply dbSelect; eauto.
+Qed.
+
+Lemma aux__se_cmd__denotes__op_cmd : forall S TD Ps F B c cs call0 sbs tmn lc arg0 als ECs gl Mem1 lc' gl' als' Mem2 lc0 gl0 als0 Mem0 sstate1 tr1 tr2,
+  uniq sstate1.(STerms) ->
+  (dom lc0 `union` dom gl0) [<=] dom (STerms sstate1) ->
+  sstate_denotes_state TD lc0 gl0 als0 Mem0 sstate1 lc gl als Mem1 tr1 ->
+  sstate_denotes_state TD lc0 gl0 als0 Mem0 (se_cmd sstate1 c) lc' gl' als' Mem2 tr2 ->
+  exists tr,
+    dbCmd (mkState S TD Ps ((mkEC F B ((subblock_intro (c::cs) call0)::sbs) tmn lc arg0 als)::ECs) gl Mem1)
+          (mkState S TD Ps ((mkEC F B ((subblock_intro cs call0)::sbs) tmn lc' arg0 als')::ECs) gl' Mem2)
+          tr /\
+    tr2 = trace_app tr1 tr.
+Proof.
+  intros S TD Ps F B c cs call0 sbs tmn lc arg0 als ECs gl Mem1 lc' gl' als' Mem2 lc0 gl0 als0 Mem0 sstate1 tr1 tr2 Huniq Hsub Hdenotes1 Hdenotes2.
+  assert (J:=Hdenotes2).
+  apply aux__se_cmd__denotes__exists_op_cmd with
+    (S:=S)(Ps:=Ps)(F:=F)(B:=B)(cs:=cs)(call0:=call0)(sbs:=sbs)(tmn:=tmn)(lc:=lc)
+    (arg0:=arg0)(als:=als)(ECs:=ECs)(gl:=gl)(Mem1:=Mem1)(tr1:=tr1) in J; simpl; auto.
+  destruct J as [lc'' [gl'' [als'' [Mem2' [tr [HdbCmd EQ]]]]]]; subst.
+  exists tr. split; auto.
+  assert (Hdenotes2':=HdbCmd).
+  apply op_cmd__satisfies__se_cmd with (lc0:=lc0)(gl0:=gl0)(als0:=als0)(Mem0:=Mem0)(sstate1:=sstate1)(tr1:=tr1) in Hdenotes2'; auto.
+  apply sstate_denotes_state_det with (lc2:=lc')(gl2:=gl')(als2:=als')(Mem2:=Mem2)(tr2:=trace_app tr1 tr) in Hdenotes2'; auto.
+  destruct Hdenotes2' as [EQ1 [EQ2 [EQ3 EQ4]]]; subst.
+  eapply dbCmd_eqEnv; eauto.
+Qed.
+
+Lemma se_cmd__denotes__op_cmd : forall S TD Ps F B c cs call0 sbs tmn lc arg0 als ECs gl Mem1 lc' gl' als' Mem2 tr,
+  uniq gl ->
+  uniq lc ->
+  sstate_denotes_state TD lc gl als Mem1 (se_cmd (mkSstate (env_to_smap gl lc) smem_init sframe_init nil) c) lc' gl' als' Mem2 tr ->
+  dbCmd (mkState S TD Ps ((mkEC F B ((subblock_intro (c::cs) call0)::sbs) tmn lc arg0 als)::ECs) gl Mem1)
+        (mkState S TD Ps ((mkEC F B ((subblock_intro cs call0)::sbs) tmn lc' arg0 als')::ECs) gl' Mem2)
+        tr. 
+Proof.
+  intros S TD Ps F B c cs call0 sbs tmn lc arg0 als ECs gl Mem1 lc' gl' als' Mem2 tr Huniqg Huniqc Hdenotes.
+  assert (J:=Hdenotes).
+  apply aux__se_cmd__denotes__op_cmd with
+    (lc:=lc)(gl:=gl)(Mem1:=Mem1)(tr1:=trace_nil)(call0:=call0)(sbs:=sbs)(tmn:=tmn)(als:=als)
+    (S:=S)(Ps:=Ps)(F:=F)(B:=B)(cs:=cs)(arg0:=arg0)(ECs:=ECs) in J; simpl; auto.
+    simpl in J. destruct J as [tr0 [J1 J2]]; subst; auto.
+    apply env_to_smap_uniq.
+    rewrite env_to_smap_dom_eq. fsetdec.
+    apply env_to_smap_denotes_id; auto.
+Qed.
+
+Lemma ssa_se_cmd : forall i0 st0 smap1 smem1 sframe1 seffects1 c,
+  binds i0 st0 smap1 ->
+  binds i0 st0 (STerms (se_cmd (mkSstate smap1 smem1 sframe1 seffects1) c)).
+  (* SSA *)
+Admitted.
+
+Lemma ssa_se_cmds : forall i0 st0 smap1 smem1 sframe1 seffects1 cs,
+  binds i0 st0 smap1 ->
+  binds i0 st0 (STerms (se_cmds (mkSstate smap1 smem1 sframe1 seffects1) cs)).
+  (* SSA *)
+Admitted.
+
+Lemma se_cmds_denotes__decomposes__head : forall c TD lc0 gl0 als0 Mem0 cs lc2 gl2 als2 Mem2 tr,
+  uniq gl0 ->
+  uniq lc0 ->
+  sstate_denotes_state TD lc0 gl0 als0 Mem0 (se_cmds (se_cmd (mkSstate (env_to_smap gl0 lc0) smem_init sframe_init nil) c) cs) lc2 gl2 als2 Mem2 tr ->
+  exists lc1, exists gl1, exists als1, exists Mem1, exists tr1,
+    sstate_denotes_state TD lc0 gl0 als0 Mem0 (se_cmd (mkSstate (env_to_smap gl0 lc0) smem_init sframe_init nil) c) lc1 gl1 als1 Mem1 tr1.
+Proof.
+  intros c TD lc0 gl0 als0 Mem0 cs lc2 gl2 als2 Mem2 tr Huniqg Huniqc Hdenotes.
+  assert (Uniqi:=@env_to_smap_uniq gl0 lc0).
+  assert (union (dom lc0) (dom gl0) [<=] dom (env_to_smap gl0 lc0)) as Subi.
+    rewrite env_to_smap_dom_eq. fsetdec.
+  generalize dependent TD.
+  generalize dependent lc0.
+  generalize dependent gl0.
+  generalize dependent als0.
+  generalize dependent Mem0.
+  generalize dependent cs.
+  generalize dependent lc2.
+  generalize dependent gl2.
+  generalize dependent als2.
+  generalize dependent Mem2.
+  generalize dependent tr.
+  (cmd_cases (destruct c) Case);
+    intros;
+    destruct Hdenotes as [[Hsterms_denote1 Hsterms_denote2] [Hsmem_denotes [Hsframe_denotes Hseffects_denote]]].
+  Case "insn_bop".
+    assert (binds i0  
+             (sterm_bop b s (value2Sterm (env_to_smap gl0 lc0) v)
+                            (value2Sterm (env_to_smap gl0 lc0) v0))
+             (STerms (se_cmds (se_cmd (mkSstate (env_to_smap gl0 lc0) smem_init sframe_init nil) (insn_bop i0 b s v v0)) cs))) as J.
+      apply ssa_se_cmds.
+      simpl. apply binds_updateSmap_eq; auto.
+    apply Hsterms_denote1 in J.
+    destruct J as [gv3 [bop_denotes_gv3 gv3_in_env2]].
+    inversion bop_denotes_gv3; subst.
+    apply value2Sterm_denotes__implies__genericvalue with (lc:=lc0)(gl:=gl0) in H8; eauto using env_to_smap_denotes_gvmap.
+    apply value2Sterm_denotes__implies__genericvalue with (lc:=lc0)(gl:=gl0) in H9; eauto using env_to_smap_denotes_gvmap.
+    assert (HupdateEnv:=exists_updateEnv lc0 gl0 i0 gv3).
+    destruct HupdateEnv as [lc1 [gl1 HupdateEnv]].
+    exists lc1. exists gl1. exists als0. exists Mem0. exists trace_nil.
+    split; auto.
+        split; intros.
+          simpl in H.
+          apply updateSmap_inversion in H; auto.
+          destruct H as [[i0_isnt_id' binds_id'_st'] | [EQ1 EQ2]]; subst.
+            apply env_to_smap_denotes__imples__gv with (TD:=TD)(Mem0:=Mem0) in binds_id'_st'; auto.
+            destruct binds_id'_st' as [gv' [st'_denotes_gv' gv'_in_env0]].
+            exists gv'. split; auto.
+            apply lookupEnv_updateEnv_neq with (id1:=id') in HupdateEnv; auto.
+            rewrite <- HupdateEnv; auto.
+
+            exists gv3. split; eauto using lookupEnv_updateEnv_eq.
+
+          destruct (i0==id'); subst.
+            apply lookupEnv_updateEnv_eq in HupdateEnv.  
+            rewrite HupdateEnv in H.
+            inversion H; subst.
+            exists (sterm_bop b s (value2Sterm (env_to_smap gl0 lc0) v) (value2Sterm (env_to_smap gl0 lc0) v0)).
+            split.
+              simpl. apply binds_updateSmap_eq; auto.
+              eauto using genericvalue__implies__value2Sterm_denotes, env_to_smap_denotes_gvmap.
+
+            apply lookupEnv_updateEnv_neq with (id1:=id') in HupdateEnv; auto.
+            rewrite <- HupdateEnv in H.
+            assert (J:=H).
+            apply lookupEnv_env_to_smap in H; auto.
+            exists (sterm_val (value_id id')).
+            split; auto.
+              apply ssa_se_cmd; auto.
+Admitted.
+
+Lemma se_cmds_denotes__decomposes__prefix : forall c TD lc0 gl0 als0 Mem0 cs lc2 gl2 als2 Mem2 tr,
+  uniq gl0 ->
+  uniq lc0 ->
+  uniq gl2 ->
+  uniq lc2 ->
+  sstate_denotes_state TD lc0 gl0 als0 Mem0 (se_cmd (se_cmds (mkSstate (env_to_smap gl0 lc0) smem_init sframe_init nil) cs) c) lc2 gl2 als2 Mem2 tr ->
+  exists lc1, exists gl1, exists als1, exists Mem1, exists tr1,
+    sstate_denotes_state TD lc0 gl0 als0 Mem0 (se_cmds (mkSstate (env_to_smap gl0 lc0) smem_init sframe_init nil) cs) lc1 gl1 als1 Mem1 tr1 /\
+    uniq gl1 /\ uniq lc1.
+Proof.
+  intros c TD lc0 gl0 als0 Mem0 cs lc2 gl2 als2 Mem2 tr Huniqg0 Huniqc0 Huniqg2 Huniqc2 Hdenotes.
+  assert (uniq (STerms (se_cmds (mkSstate (env_to_smap gl0 lc0) smem_init sframe_init nil) cs))) as Uniq1.
+    eauto using env_to_smap_uniq, se_cmds_uniq.
+  generalize dependent TD.
+  generalize dependent lc0.
+  generalize dependent gl0.
+  generalize dependent als0.
+  generalize dependent Mem0.
+  generalize dependent cs.
+  generalize dependent lc2.
+  generalize dependent gl2.
+  generalize dependent als2.
+  generalize dependent Mem2.
+  generalize dependent tr.
+  (cmd_cases (destruct c) Case);
+    intros;
+    destruct Hdenotes as [[Hsterms_denote1 Hsterms_denote2] [Hsmem_denotes [Hsframe_denotes Hseffects_denote]]].
+  Case "insn_bop".
+    assert (binds i0  
+             (sterm_bop b s (value2Sterm (STerms (se_cmds (mkSstate (env_to_smap gl0 lc0) smem_init sframe_init nil) cs)) v)
+                            (value2Sterm (STerms (se_cmds (mkSstate (env_to_smap gl0 lc0) smem_init sframe_init nil) cs)) v0))
+             (STerms (se_cmd (se_cmds (mkSstate (env_to_smap gl0 lc0) smem_init sframe_init nil) cs) (insn_bop i0 b s v v0)))) as J.
+      simpl. apply binds_updateSmap_eq; auto.
+    apply Hsterms_denote1 in J.
+    destruct J as [gv3 [bop_denotes_gv3 gv3_in_env2]].
+    destruct (@exists_deleteEnv lc2 gl2 i0) as [lc1 [gl1 HdeleteEnv]].
+    simpl in Hsmem_denotes, Hsframe_denotes, Hseffects_denote.
+    exists lc1. exists gl1. exists als2. exists Mem2. exists tr.
+    assert (uniq lc1 /\ uniq gl1) as Uniq.
+      apply deleteEnv_uniq in HdeleteEnv; auto.
+    destruct Uniq as [Huniqc1 Huniqg1].
+    split; auto.
+      split; auto.
+      clear Hsmem_denotes Hsframe_denotes Hseffects_denote.
+      split; intros.
+        assert (i0 <> id') as i0_isnt_id'. 
+          admit. (*SSA*)
+        apply ssa_se_cmd with (c:=insn_bop i0 b s v v0)(smem1:=smem_init)(sframe1:=sframe_init)(seffects1:=nil) in H; auto.
+        apply Hsterms_denote1 in H.
+        destruct H as [gv' [st'_denotes_gv' id'_gv'_in_env2]].
+        apply lookupEnv_deleteEnv_neq with (id0:=id') in HdeleteEnv; auto.
+        rewrite HdeleteEnv in id'_gv'_in_env2.
+        exists gv'. split; auto.
+
+        apply lookupEnv_deleteEnv_inv with (gv:=gv')(id1:=id') in HdeleteEnv; auto.
+        destruct HdeleteEnv as [id'_in_env2 i0_isnt_id'].
+        apply Hsterms_denote2 in id'_in_env2.
+        destruct id'_in_env2 as [st' [binds_id'_st' st'_denotes_gv']].
+        exists st'. split; auto.
+          simpl in binds_id'_st'.
+          apply updateSmap_inversion in binds_id'_st'; auto. 
+            destruct binds_id'_st' as [[_ binds_id'_st'] | [i0_is_id' binds_id'_st']]; auto.
+              contradict i0_is_id'; auto.
+
+  Case "insn_extractvalue".
+    assert (binds i0  
+             (sterm_extractvalue t (value2Sterm (STerms (se_cmds (mkSstate (env_to_smap gl0 lc0) smem_init sframe_init nil) cs)) v) l0)
+             (STerms (se_cmd (se_cmds (mkSstate (env_to_smap gl0 lc0) smem_init sframe_init nil) cs) (insn_extractvalue i0 t v l0)))) as J.
+      simpl. apply binds_updateSmap_eq; auto.
+    apply Hsterms_denote1 in J.
+    destruct J as [gv3 [extracvalue_denotes_gv3 gv3_in_env2]].
+    destruct (@exists_deleteEnv lc2 gl2 i0) as [lc1 [gl1 HdeleteEnv]].
+    simpl in Hsmem_denotes, Hsframe_denotes, Hseffects_denote.
+    exists lc1. exists gl1. exists als2. exists Mem2. exists tr.
+    assert (uniq lc1 /\ uniq gl1) as Uniq.
+      apply deleteEnv_uniq in HdeleteEnv; auto.
+    destruct Uniq as [Huniqc1 Huniqg1].
+    split; auto.
+      split; auto.
+      clear Hsmem_denotes Hsframe_denotes Hseffects_denote.
+      split; intros.
+        assert (i0 <> id') as i0_isnt_id'. 
+          admit. (*SSA*)
+        apply ssa_se_cmd with (c:=insn_extractvalue i0 t v l0)(smem1:=smem_init)(sframe1:=sframe_init)(seffects1:=nil) in H; auto.
+        apply Hsterms_denote1 in H.
+        destruct H as [gv' [st'_denotes_gv' id'_gv'_in_env2]].
+        apply lookupEnv_deleteEnv_neq with (id0:=id') in HdeleteEnv; auto.
+        rewrite HdeleteEnv in id'_gv'_in_env2.
+        exists gv'. split; auto.
+
+        apply lookupEnv_deleteEnv_inv with (gv:=gv')(id1:=id') in HdeleteEnv; auto.
+        destruct HdeleteEnv as [id'_in_env2 i0_isnt_id'].
+        apply Hsterms_denote2 in id'_in_env2.
+        destruct id'_in_env2 as [st' [binds_id'_st' st'_denotes_gv']].
+        exists st'. split; auto.
+          simpl in binds_id'_st'.
+          apply updateSmap_inversion in binds_id'_st'; auto. 
+            destruct binds_id'_st' as [[_ binds_id'_st'] | [i0_is_id' binds_id'_st']]; auto.
+              contradict i0_is_id'; auto.
+        
+  Case "insn_insertvalue". admit.
+
+  Case "insn_malloc".
+    assert (binds i0  
+             (sterm_malloc (SMem (se_cmds (mkSstate (env_to_smap gl0 lc0) smem_init sframe_init nil) cs)) t s a)
+             (STerms (se_cmd (se_cmds (mkSstate (env_to_smap gl0 lc0) smem_init sframe_init nil) cs) (insn_malloc i0 t s a)))) as J.
+      simpl. apply binds_updateSmap_eq; auto.
+    apply Hsterms_denote1 in J.
+    destruct J as [gv3 [malloc_denotes_gv3 gv3_in_env2]].
+    destruct (@exists_deleteEnv lc2 gl2 i0) as [lc1 [gl1 HdeleteEnv]].
+    simpl in Hsmem_denotes, Hsframe_denotes, Hseffects_denote.
+    inversion Hsmem_denotes; subst.
+    exists lc1. exists gl1. exists als2. exists Mem3. exists tr.
+    assert (uniq lc1 /\ uniq gl1) as Uniq.
+      apply deleteEnv_uniq in HdeleteEnv; auto.
+    destruct Uniq as [Huniqc1 Huniqg1].
+    split; auto.
+      split; auto.
+      clear Hsmem_denotes Hsframe_denotes Hseffects_denote.
+      split; intros.
+        assert (i0 <> id') as i0_isnt_id'. 
+          admit. (*SSA*)
+        apply ssa_se_cmd with (c:=insn_malloc i0 t s a)(smem1:=(SMem (se_cmds (mkSstate (env_to_smap gl0 lc0) smem_init sframe_init nil) cs)))(sframe1:=sframe_init)(seffects1:=nil) in H; auto.
+        apply Hsterms_denote1 in H.
+        destruct H as [gv' [st'_denotes_gv' id'_gv'_in_env2]].
+        apply lookupEnv_deleteEnv_neq with (id0:=id') in HdeleteEnv; auto.
+        rewrite HdeleteEnv in id'_gv'_in_env2.
+        exists gv'. split; auto.
+
+        apply lookupEnv_deleteEnv_inv with (gv:=gv')(id1:=id') in HdeleteEnv; auto.
+        destruct HdeleteEnv as [id'_in_env2 i0_isnt_id'].
+        apply Hsterms_denote2 in id'_in_env2.
+        destruct id'_in_env2 as [st' [binds_id'_st' st'_denotes_gv']].
+        exists st'. split; auto.
+          simpl in binds_id'_st'.
+          apply updateSmap_inversion in binds_id'_st'; auto. 
+            destruct binds_id'_st' as [[_ binds_id'_st'] | [i0_is_id' binds_id'_st']]; auto.
+              contradict i0_is_id'; auto.
+    
+  Case "insn_free".
+    simpl in Hsmem_denotes, Hsframe_denotes, Hseffects_denote.
+    inversion Hsmem_denotes; subst.
+    exists lc2. exists gl2. exists als2. exists Mem3. exists tr.
+    split; auto.
+      split; auto.
+      clear Hsmem_denotes Hsframe_denotes Hseffects_denote.
+      split; intros.
+        apply ssa_se_cmd with (c:=insn_free i0 t v)(smem1:=(SMem (se_cmds (mkSstate (env_to_smap gl0 lc0) smem_init sframe_init nil) cs)))(sframe1:=sframe_init)(seffects1:=nil) in H; auto.
+
+        apply Hsterms_denote2 in H.
+        destruct H as [st' [binds_id'_st' st'_denotes_gv']].
+        exists st'. split; auto.
+
+  Case "insn_alloca".
+    assert (binds i0  
+             (sterm_alloca (SMem (se_cmds (mkSstate (env_to_smap gl0 lc0) smem_init sframe_init nil) cs)) t s a)
+             (STerms (se_cmd (se_cmds (mkSstate (env_to_smap gl0 lc0) smem_init sframe_init nil) cs) (insn_alloca i0 t s a)))) as J.
+      simpl. apply binds_updateSmap_eq; auto.
+    apply Hsterms_denote1 in J.
+    destruct J as [gv3 [alloca_denotes_gv3 gv3_in_env2]].
+    destruct (@exists_deleteEnv lc2 gl2 i0) as [lc1 [gl1 HdeleteEnv]].
+    simpl in Hsmem_denotes, Hsframe_denotes, Hseffects_denote.
+    inversion Hsmem_denotes; subst.
+    inversion Hsframe_denotes; subst.
+    exists lc1. exists gl1. exists (als3). exists Mem3. exists tr.
+    assert (uniq lc1 /\ uniq gl1) as Uniq.
+      apply deleteEnv_uniq in HdeleteEnv; auto.
+    destruct Uniq as [Huniqc1 Huniqg1].
+    split; auto.
+      split; auto.
+      clear Hsmem_denotes Hsframe_denotes Hseffects_denote.
+      split; intros.
+        assert (i0 <> id') as i0_isnt_id'. 
+          admit. (*SSA*)
+        apply ssa_se_cmd with (c:=insn_alloca i0 t s a)(smem1:=(SMem (se_cmds (mkSstate (env_to_smap gl0 lc0) smem_init sframe_init nil) cs)))(sframe1:=sframe_init)(seffects1:=nil) in H; auto.
+        apply Hsterms_denote1 in H.
+        destruct H as [gv' [st'_denotes_gv' id'_gv'_in_env2]].
+        apply lookupEnv_deleteEnv_neq with (id0:=id') in HdeleteEnv; auto.
+        rewrite HdeleteEnv in id'_gv'_in_env2.
+        exists gv'. split; auto.
+
+        apply lookupEnv_deleteEnv_inv with (gv:=gv')(id1:=id') in HdeleteEnv; auto.
+        destruct HdeleteEnv as [id'_in_env2 i0_isnt_id'].
+        apply Hsterms_denote2 in id'_in_env2.
+        destruct id'_in_env2 as [st' [binds_id'_st' st'_denotes_gv']].
+        exists st'. split; auto.
+          simpl in binds_id'_st'.
+          apply updateSmap_inversion in binds_id'_st'; auto. 
+            destruct binds_id'_st' as [[_ binds_id'_st'] | [i0_is_id' binds_id'_st']]; auto.
+              contradict i0_is_id'; auto.
+Admitted.
+
+Lemma se_cmds_denotes__decomposes__prefix_last : forall c TD lc0 gl0 als0 Mem0 cs lc2 gl2 als2 Mem2 tr,
+  uniq gl0 ->
+  uniq lc0 ->
+  uniq gl2 ->
+  uniq lc2 ->
+  sstate_denotes_state TD lc0 gl0 als0 Mem0 (se_cmd (se_cmds (mkSstate (env_to_smap gl0 lc0) smem_init sframe_init nil) cs) c) lc2 gl2 als2 Mem2 tr ->
+  exists lc1, exists gl1, exists als1, exists Mem1, exists tr1, exists tr2,
+    sstate_denotes_state TD lc0 gl0 als0 Mem0 (se_cmds (mkSstate (env_to_smap gl0 lc0) smem_init sframe_init nil) cs) lc1 gl1 als1 Mem1 tr1 /\
+    sstate_denotes_state TD lc1 gl1 als1 Mem1 (se_cmd (mkSstate (env_to_smap gl1 lc1) smem_init sframe_init nil) c) lc2 gl2 als2 Mem2 tr2 /\
+    tr = trace_app tr1 tr2 /\ 
+    uniq gl1 /\ uniq lc1.
+Proof.
+  intros c TD lc0 gl0 als0 Mem0 cs lc2 gl2 als2 Mem2 tr Huniqg0 Huniqc0 Huniqg2 Huniqc2 Hdenotes.
+  assert (uniq (STerms (se_cmds (mkSstate (env_to_smap gl0 lc0) smem_init sframe_init nil) cs))) as Uniq1.
+    eauto using env_to_smap_uniq, se_cmds_uniq.
+  assert (Hsub:=@se_cmds_env_to_smap_dom_sub lc0 gl0 cs).
+  generalize dependent TD.
+  generalize dependent lc0.
+  generalize dependent gl0.
+  generalize dependent als0.
+  generalize dependent Mem0.
+  generalize dependent cs.
+  generalize dependent lc2.
+  generalize dependent gl2.
+  generalize dependent als2.
+  generalize dependent Mem2.
+  generalize dependent tr.
+  (cmd_cases (destruct c) Case);
+    intros;
+    destruct Hdenotes as [[Hsterms_denote1 Hsterms_denote2] [Hsmem_denotes [Hsframe_denotes Hseffects_denote]]].
+  Case "insn_bop".
+    assert (binds i0  
+             (sterm_bop b s (value2Sterm (STerms (se_cmds (mkSstate (env_to_smap gl0 lc0) smem_init sframe_init nil) cs)) v)
+                            (value2Sterm (STerms (se_cmds (mkSstate (env_to_smap gl0 lc0) smem_init sframe_init nil) cs)) v0))
+             (STerms (se_cmd (se_cmds (mkSstate (env_to_smap gl0 lc0) smem_init sframe_init nil) cs) (insn_bop i0 b s v v0)))) as J.
+      simpl. apply binds_updateSmap_eq; auto.
+    apply Hsterms_denote1 in J.
+    destruct J as [gv3 [bop_denotes_gv3 gv3_in_env2]].
+    destruct (@exists_deleteEnv lc2 gl2 i0) as [lc1 [gl1 HdeleteEnv]].
+    simpl in Hsmem_denotes, Hsframe_denotes, Hseffects_denote.
+    exists lc1. exists gl1. exists als2. exists Mem2. exists tr. exists trace_nil.
+    rewrite trace_app_nil__eq__trace.
+    assert (uniq lc1 /\ uniq gl1) as Uniq.
+      apply deleteEnv_uniq in HdeleteEnv; auto.
+    destruct Uniq as [Huniqc1 Huniqg1].
+    assert (smap_denotes_gvmap TD lc0 gl0 Mem0
+              (STerms (se_cmds (mkSstate (env_to_smap gl0 lc0) smem_init sframe_init nil) cs))
+              lc1 gl1) as env0_denote_env1.
+      clear Hsmem_denotes Hsframe_denotes Hseffects_denote.
+      split; intros.
+        assert (i0 <> id') as i0_isnt_id'. 
+          admit. (*SSA*)
+        apply ssa_se_cmd with (c:=insn_bop i0 b s v v0)(smem1:=smem_init)(sframe1:=sframe_init)(seffects1:=nil) in H; auto.
+        apply Hsterms_denote1 in H.
+        destruct H as [gv' [st'_denotes_gv' id'_gv'_in_env2]].
+        apply lookupEnv_deleteEnv_neq with (id0:=id') in HdeleteEnv; auto.
+        rewrite HdeleteEnv in id'_gv'_in_env2.
+        exists gv'. split; auto.
+
+        apply lookupEnv_deleteEnv_inv with (gv:=gv')(id1:=id') in HdeleteEnv; auto.
+        destruct HdeleteEnv as [id'_in_env2 i0_isnt_id'].
+        apply Hsterms_denote2 in id'_in_env2.
+        destruct id'_in_env2 as [st' [binds_id'_st' st'_denotes_gv']].
+        exists st'. split; auto.
+          simpl in binds_id'_st'.
+          apply updateSmap_inversion in binds_id'_st'; auto. 
+            destruct binds_id'_st' as [[_ binds_id'_st'] | [i0_is_id' binds_id'_st']]; auto.
+              contradict i0_is_id'; auto.
+    split.
+      split; auto.
+    split; auto.
+      split; auto.
+        split; intros.
+          simpl in H.
+          apply updateSmap_inversion in H; auto using env_to_smap_uniq.
+          destruct H as [[i0_isnt_id' binds_id'_st'] | [EQ1 EQ2]]; subst.
+            apply env_to_smap_denotes__imples__gv with (TD:=TD)(Mem0:=Mem2) in binds_id'_st'; auto.
+            destruct binds_id'_st' as [gv' [st'_denotes_gv' gv'_in_env1]].
+            exists gv'. split; auto.
+            apply lookupEnv_deleteEnv_neq with (id0:=id') in HdeleteEnv; auto.
+            rewrite HdeleteEnv; auto.
+
+            exists gv3. split; eauto using lookupEnv_deleteEnv_eq.
+            clear Hsmem_denotes Hsframe_denotes Hseffects_denote.
+            inversion bop_denotes_gv3; subst. clear bop_denotes_gv3.
+            apply sterm_bop_denotes with (gv1:=gv1)(gv2:=gv2); auto.
+              apply value2Sterm_denotes__implies__genericvalue with (lc:=lc1)(gl:=gl1) in H8; auto.
+                apply genericvalue__implies__value2Sterm_denotes with (lc:=lc1)(gl:=gl1); auto using env_to_smap_uniq.
+                  apply env_to_smap_denotes_gvmap; auto.
+              apply value2Sterm_denotes__implies__genericvalue with (lc:=lc1)(gl:=gl1) in H9; auto.
+                apply genericvalue__implies__value2Sterm_denotes with (lc:=lc1)(gl:=gl1); auto using env_to_smap_uniq.
+                  apply env_to_smap_denotes_gvmap; auto.
+
+          assert (id'_in_env2:=H).
+          apply Hsterms_denote2 in H.
+          destruct H as [st' [binds_id'_st' st'_denotes_gv']].
+          simpl in binds_id'_st'.
+          apply updateSmap_inversion in binds_id'_st'; auto. 
+            destruct binds_id'_st' as [[i0_isnt_id' binds_id'_st'] | [i0_is_id' binds_id'_st']]; subst.
+              apply lookupEnv_deleteEnv_neq with (id0:=id') in HdeleteEnv; auto.
+              rewrite HdeleteEnv in id'_in_env2.              
+              exists (sterm_val (value_id id')).
+              clear Hsmem_denotes Hsframe_denotes Hseffects_denote.
+              split; auto.
+                simpl.
+                apply binds_updateSmap_neq; auto.
+                apply lookupEnv_env_to_smap with (gv0:=gv'); auto.
+
+              rewrite id'_in_env2 in gv3_in_env2.
+              inversion gv3_in_env2; subst. clear gv3_in_env2.
+              simpl.
+              exists (sterm_bop b s (value2Sterm (env_to_smap gl1 lc1) v) (value2Sterm (env_to_smap gl1 lc1) v0)).
+              split; auto using binds_updateSmap_eq.
+                inversion bop_denotes_gv3; subst.
+                apply sterm_bop_denotes with (gv1:=gv1)(gv2:=gv2); auto.
+                  apply value2Sterm_denotes__implies__genericvalue with (lc:=lc1)(gl:=gl1) in H8; auto.
+                    apply genericvalue__implies__value2Sterm_denotes with (lc:=lc1)(gl:=gl1); auto using env_to_smap_uniq.
+                      apply env_to_smap_denotes_gvmap; auto.
+                  apply value2Sterm_denotes__implies__genericvalue with (lc:=lc1)(gl:=gl1) in H9; auto.
+                    apply genericvalue__implies__value2Sterm_denotes with (lc:=lc1)(gl:=gl1); auto using env_to_smap_uniq.
+                      apply env_to_smap_denotes_gvmap; auto.
+
+Admitted.
+
+Lemma se_cmds_denotes__composes__prefix_last : forall c TD lc1 gl1 als1 Mem1 
+  lc2 gl2 als2 Mem2 lc0 gl0 als0 Mem0 tr1 tr2 cs,
+  uniq lc1 ->
+  uniq gl1 ->
+  sstate_denotes_state TD lc0 gl0 als0 Mem0 (se_cmds (mkSstate (env_to_smap gl0 lc0) smem_init sframe_init nil) cs) lc1 gl1 als1 Mem1 tr1 ->
+  sstate_denotes_state TD lc1 gl1 als1 Mem1 (se_cmd (mkSstate (env_to_smap gl1 lc1) smem_init sframe_init nil) c) lc2 gl2 als2 Mem2 tr2 ->
+  sstate_denotes_state TD lc0 gl0 als0 Mem0 (se_cmds (mkSstate (env_to_smap gl0 lc0) smem_init sframe_init nil) (cs++c::nil)) lc2 gl2 als2 Mem2 (trace_app tr1 tr2).
+Proof.
+  intros c TD lc1 gl1 als1 Mem1 lc2 gl2 als2 Mem2 lc0 gl0 als0 Mem0 tr1 tr2 cs Huniqc1 Huniqg1 Hdenotes1 Hdenotes2.
+  assert (uniq (STerms (se_cmds (mkSstate (env_to_smap gl0 lc0) smem_init sframe_init nil) cs))) as Uniq1.
+    eauto using env_to_smap_uniq, se_cmds_uniq.
+  generalize dependent TD.
+  generalize dependent lc0.
+  generalize dependent gl0.
+  generalize dependent als0.
+  generalize dependent Mem0.
+  generalize dependent cs.
+  generalize dependent lc2.
+  generalize dependent gl2.
+  generalize dependent als2.
+  generalize dependent Mem2.
+  generalize dependent lc1.
+  generalize dependent gl1.
+  generalize dependent als1.
+  generalize dependent Mem1.
+  generalize dependent tr1.
+  generalize dependent tr2.
+  (cmd_cases (destruct c) Case);
+    intros;
+    destruct Hdenotes1 as [[Hsterms_denote11 Hsterms_denote12] [Hsmem_denotes1 [Hsframe_denotes1 Hseffects_denote1]]];
+    destruct Hdenotes2 as [[Hsterms_denote21 Hsterms_denote22] [Hsmem_denotes2 [Hsframe_denotes2 Hseffects_denote2]]];
+    rewrite se_cmds_rev_cons.
+  Case "insn_bop".
+    split.
+      clear Hsmem_denotes1 Hsframe_denotes1 Hseffects_denote1 Hsmem_denotes2 Hsframe_denotes2 Hseffects_denote2.
+      split; intros.
+        simpl in H.
+        apply updateSmap_inversion in H; auto. 
+          destruct H as [[i0_isnt_id' binds_id'_st'] | [i0_is_id' binds_id'_st']]; subst.
+            apply Hsterms_denote11 in binds_id'_st'.
+            destruct binds_id'_st' as [gv' [st'_denotes_gv' id'_gv'_in_env1]].
+            exists gv'. split; auto.
+              admit. (*SSA*)
+
+            assert (binds id' (sterm_bop b s (value2Sterm (env_to_smap gl1 lc1) v) (value2Sterm (env_to_smap gl1 lc1) v0))
+                    (STerms (se_cmd (mkSstate (env_to_smap gl1 lc1) smem_init sframe_init nil) (insn_bop id' b s v v0)))
+            ) as binds_id'_bop.
+              simpl. apply binds_updateSmap_eq; auto.
+            apply Hsterms_denote21 in binds_id'_bop.
+            destruct binds_id'_bop as [gv' [bop_denotes_gv' id'_gv'_in_env2]].
+            exists gv'. split; auto.
+              inversion bop_denotes_gv'; subst.
+              apply sterm_bop_denotes with (gv1:=gv1)(gv2:=gv2); auto.
+                apply value2Sterm_denotes__implies__genericvalue with (lc:=lc1)(gl:=gl1) in H8; auto.
+                  apply genericvalue__implies__value2Sterm_denotes with (lc:=lc1)(gl:=gl1); auto using env_to_smap_uniq.
+                    split; auto.
+                  apply env_to_smap_uniq.
+                  rewrite env_to_smap_dom_eq. fsetdec.
+                  apply env_to_smap_denotes_gvmap; auto.
+                apply value2Sterm_denotes__implies__genericvalue with (lc:=lc1)(gl:=gl1) in H9; auto.
+                  apply genericvalue__implies__value2Sterm_denotes with (lc:=lc1)(gl:=gl1); auto using env_to_smap_uniq.
+                    split; auto.
+                  apply env_to_smap_uniq.
+                  rewrite env_to_smap_dom_eq. fsetdec.
+                  apply env_to_smap_denotes_gvmap; auto.
+
+        apply Hsterms_denote22 in H.
+        destruct H as [st' [binds_id'_st' st'_denotes_gv']].
+        simpl in binds_id'_st'.
+        apply updateSmap_inversion in binds_id'_st'; auto using env_to_smap_uniq.
+        destruct binds_id'_st' as [[i0_isnt_id' binds_id'_st'] | [i0_is_id' binds_id'_st']]; subst.
+          apply binds_env_to_smap with (TD:=TD) in binds_id'_st'; auto.
+            destruct binds_id'_st' as [EQ [gv id'_gv_in_env1]]; subst.
+            assert (J:=id'_gv_in_env1).
+            unfold getOperandValue in J.
+            apply Hsterms_denote12 in J.
+            destruct J as [st' [binds_id'_st' st'_denotes_gv]].
+            inversion st'_denotes_gv'; subst.
+            rewrite id'_gv_in_env1 in H4.
+            inversion H4; subst. clear H4.
+            exists st'.
+            split; auto.
+              simpl.
+              apply binds_updateSmap_neq; auto.
+
+          exists (sterm_bop b s 
+                   (value2Sterm (STerms (se_cmds (mkSstate (env_to_smap gl0 lc0) smem_init sframe_init nil) cs)) v)
+                   (value2Sterm (STerms (se_cmds (mkSstate (env_to_smap gl0 lc0) smem_init sframe_init nil) cs)) v0)).
+          split.
+            simpl. apply binds_updateSmap_eq; auto.
+            inversion st'_denotes_gv'; subst.
+            apply sterm_bop_denotes with (gv1:=gv1)(gv2:=gv2); auto.
+              apply value2Sterm_denotes__implies__genericvalue with (lc:=lc1)(gl:=gl1) in H8; auto.
+                apply genericvalue__implies__value2Sterm_denotes with (lc:=lc1)(gl:=gl1); auto using env_to_smap_uniq.
+                  split; auto.
+                apply env_to_smap_uniq.
+                rewrite env_to_smap_dom_eq. fsetdec.
+                apply env_to_smap_denotes_gvmap; auto.
+              apply value2Sterm_denotes__implies__genericvalue with (lc:=lc1)(gl:=gl1) in H9; auto.
+                apply genericvalue__implies__value2Sterm_denotes with (lc:=lc1)(gl:=gl1); auto using env_to_smap_uniq.
+                  split; auto.
+                apply env_to_smap_uniq.
+                rewrite env_to_smap_dom_eq. fsetdec.
+                apply env_to_smap_denotes_gvmap; auto.
+    split.
+      clear Hsframe_denotes1 Hseffects_denote1 Hsframe_denotes2 Hseffects_denote2.
+      clear Hsterms_denote11 Hsterms_denote12 Hsterms_denote21 Hsterms_denote22.
+      simpl in *.
+      inversion Hsmem_denotes2; subst; auto.
+    split.
+      clear Hsmem_denotes1 Hseffects_denote1 Hsmem_denotes2 Hseffects_denote2.
+      clear Hsterms_denote11 Hsterms_denote12 Hsterms_denote21 Hsterms_denote22.
+      simpl in *.
+      inversion Hsframe_denotes2; subst; auto.
+
+      clear Hsmem_denotes1 Hsframe_denotes1 Hsmem_denotes2 Hsframe_denotes2.
+      clear Hsterms_denote11 Hsterms_denote12 Hsterms_denote21 Hsterms_denote22.
+      simpl in *.
+      inversion Hseffects_denote1; subst.      
+      inversion Hseffects_denote2; subst; auto.  
+Admitted.
+
+Definition se_cmds_denotes__decomposes__app_prop (cs2:list cmd) :=
+forall TD lc0 gl0 als0 Mem0 cs1 lc2 gl2 als2 Mem2 tr,
+  uniq gl0 ->
+  uniq lc0 ->
+  uniq gl2 ->
+  uniq lc2 ->
+  sstate_denotes_state TD lc0 gl0 als0 Mem0 (se_cmds (mkSstate (env_to_smap gl0 lc0) smem_init sframe_init nil) (cs1++cs2)) lc2 gl2 als2 Mem2 tr ->
+  exists lc1, exists gl1, exists als1, exists Mem1, exists tr1, exists tr2,
+    sstate_denotes_state TD lc0 gl0 als0 Mem0 (se_cmds (mkSstate (env_to_smap gl0 lc0) smem_init sframe_init nil) cs1) lc1 gl1 als1 Mem1 tr1 /\
+    sstate_denotes_state TD lc1 gl1 als1 Mem1 (se_cmds (mkSstate (env_to_smap gl1 lc1) smem_init sframe_init nil) cs2) lc2 gl2 als2 Mem2 tr2 /\
+    tr = trace_app tr1 tr2 /\ uniq gl1 /\ uniq lc1.
+
+Lemma se_cmds_denotes__decomposes__app : forall cs2, 
+  se_cmds_denotes__decomposes__app_prop cs2.
+Proof.
+  apply (@rev_ind cmd); unfold se_cmds_denotes__decomposes__app_prop in *; intros; simpl.
+  Case "nil".
+    exists lc2. exists gl2. exists als2. exists Mem2. exists tr. exists trace_nil.
+    rewrite trace_app_nil__eq__trace.
+    rewrite <- app_nil_end in H3.
+    split; auto.
+    split; auto.
+      apply env_to_smap_denotes_id; auto.
+  Case "cons".
+    rewrite <- app_ass in H4.
+    rewrite se_cmds_rev_cons in H4.
+    apply se_cmds_denotes__decomposes__prefix_last in H4; auto.
+    destruct H4 as [lc1 [gl1 [als1 [Mem1 [tr1 [tr2 [env0_denotes_env1 [env1_denotes_env2 [EQ [Huniqg1 Huniqc1]]]]]]]]]]; subst.
+    apply H in env0_denotes_env1; auto.
+    destruct env0_denotes_env1 as [lc3 [gl3 [als3 [Mem3 [tr3 [tr4 [env0_denotes_env3 [env3_denotes_env1 [EQ [Huniqg3 Huniqc3]]]]]]]]]]; subst.
+    exists lc3. exists gl3. exists als3. exists Mem3. exists tr3. exists (trace_app tr4 tr2).
+    rewrite trace_app_commute.
+    split; auto.
+    split; auto.
+     apply se_cmds_denotes__composes__prefix_last with (lc1:=lc1)(gl1:=gl1)(als1:=als1)(Mem1:=Mem1); eauto.
+Qed.
+
+Lemma se_cmds_denotes__decomposes__head_tail : forall c TD lc0 gl0 als0 Mem0 cs lc2 gl2 als2 Mem2 tr,
+  uniq gl0 ->
+  uniq lc0 ->
+  uniq gl2 ->
+  uniq lc2 ->
+  sstate_denotes_state TD lc0 gl0 als0 Mem0 (se_cmds (se_cmd (mkSstate (env_to_smap gl0 lc0) smem_init sframe_init nil) c) cs) lc2 gl2 als2 Mem2 tr ->
+  exists lc1, exists gl1, exists als1, exists Mem1, exists tr1, exists tr2,
+    sstate_denotes_state TD lc0 gl0 als0 Mem0 (se_cmd (mkSstate (env_to_smap gl0 lc0) smem_init sframe_init nil) c) lc1 gl1 als1 Mem1 tr1 /\
+    sstate_denotes_state TD lc1 gl1 als1 Mem1 (se_cmds (mkSstate (env_to_smap gl1 lc1) smem_init sframe_init nil) cs) lc2 gl2 als2 Mem2 tr2 /\
+    tr = trace_app tr1 tr2 /\ uniq gl1 /\ uniq lc1.
+Proof.
+  intros c TD lc0 gl0 als0 Mem0 cs lc2 gl2 als2 Mem2 tr Huniqg0 Huniqc0 Huniqg2 Huniqc2 Hdenotes.
+  rewrite <- se_cmds_cons in Hdenotes.
+  apply se_cmds_denotes__decomposes__app in Hdenotes; auto.
+Qed.    
+  
+Lemma se_cmds__denote__exists_op_cmds : forall cs S TD Ps F B call0 sbs tmn lc1 arg als1 ECs gl1 Mem1 lc2 gl2 als2 Mem2 tr,
+  uniq gl1 ->
+  uniq lc1 ->
+  uniq gl2 ->
+  uniq lc2 ->
+  sstate_denotes_state TD lc1 gl1 als1 Mem1 (se_cmds (mkSstate (env_to_smap gl1 lc1) smem_init sframe_init nil) cs) lc2 gl2 als2 Mem2 tr ->
+  exists lc2', exists gl2', exists als2, exists Mem2', exists tr', 
+    dbCmds (mkState S TD Ps ((mkEC F B ((subblock_intro cs call0)::sbs) tmn lc1 arg als1)::ECs) gl1 Mem1)
+           (mkState S TD Ps ((mkEC F B ((subblock_intro nil call0)::sbs) tmn lc2' arg als2)::ECs) gl2' Mem2')
+           tr'.
+Proof.
+  induction cs; 
+    intros S TD Ps F B call0 sbs tmn lc1 arg0 als1 ECs gl1 Mem1 lc2 gl2 als2 Mem2 tr Uniqg1 Uniqc1 Uniqg2 Uniqc2 Hdenotes.
+
+    simpl in *. 
+    exists lc1. exists gl1. exists als1. exists Mem2. exists trace_nil. 
+    assert (J:=@env_to_smap_denotes_id TD lc1 gl1 als1 Mem1 Uniqg1 Uniqc1).
+    apply sstate_denotes_state_det with (lc2:=lc2)(gl2:=gl2)(als2:=als2)(Mem2:=Mem2)(tr2:=tr) in J; auto.
+    destruct J as [EQ1 [EQ2 [EQ3 EQ4]]]; subst; auto.
+
+    simpl in Hdenotes.
+    apply se_cmds_denotes__decomposes__head_tail in Hdenotes; auto.
+    destruct Hdenotes as [lc3 [gl3 [als3 [Mem3 [tr3 [tr3' [J1 [J2 [EQ [Huniqg3 Huniqc3]]]]]]]]]]; subst.
+    apply se_cmd__denotes__op_cmd with
+      (S:=S)(Ps:=Ps)(F:=F)(B:=B)(cs:=cs)(call0:=call0)(sbs:=sbs)(tmn:=tmn)(lc:=lc1)
+     (arg0:=arg0)(als:=als1)(ECs:=ECs)(gl:=gl1)(Mem1:=Mem1) in J1; simpl; auto.
+    apply IHcs with
+      (S:=S)(Ps:=Ps)(F:=F)(B:=B)(call0:=call0)(sbs:=sbs)(tmn:=tmn)
+      (arg:=arg0)(ECs:=ECs) in J2; simpl; auto.
+      destruct J2 as [lc4 [gl4 [als4 [Mem4 [tr4 HdbCmds]]]]].
+      exists lc4. exists gl4. exists als4. exists Mem4. exists (trace_app tr3 tr4). 
+      apply dbCmds_cons with (S2:=mkState S TD Ps ((mkEC F B (subblock_intro cs call0::sbs) tmn lc3 arg0 als3)::ECs) gl3 Mem3); eauto.
+Qed.
+
+Lemma se_cmds__denote__op_cmds : forall S TD Ps F B cs call0 sbs tmn lc1 arg ECs gl1 als1 Mem1 lc2 als2 gl2 Mem2 tr,
+  uniq gl1 ->
+  uniq lc1 ->
+  uniq gl2 ->
+  uniq lc2 ->
+  sstate_denotes_state TD lc1 gl1 als1 Mem1 (se_cmds (mkSstate (env_to_smap gl1 lc1) smem_init sframe_init nil) cs) lc2 gl2 als2 Mem2 tr ->
+  dbCmds (mkState S TD Ps ((mkEC F B ((subblock_intro cs call0)::sbs) tmn lc1 arg als1)::ECs) gl1 Mem1)
+         (mkState S TD Ps ((mkEC F B ((subblock_intro nil call0)::sbs) tmn lc2 arg als2)::ECs) gl2 Mem2)
+         tr. 
+Proof.
+  intros S TD Ps F B cs call0 sbs tmn lc1 arg0 ECs gl1 als1 Mem1 lc2 als2 gl2 Mem2 tr Huniqg1 Huniqc1 Huniqg2 Huniqc2 Hdenotes.
+  assert (J:=Hdenotes).
+  apply se_cmds__denote__exists_op_cmds with
+    (S:=S)(Ps:=Ps)(F:=F)(B:=B)(cs:=cs)(call0:=call0)(sbs:=sbs)(tmn:=tmn)(lc1:=lc1)
+    (arg:=arg0)(als1:=als1)(ECs:=ECs)(gl1:=gl1)(Mem1:=Mem1) in J; simpl; auto.
+  destruct J as [lc2' [gl2' [als2' [Mem2' [tr' HdbCmds]]]]].
+  assert (Hdenotes':=HdbCmds).
+  apply op_cmds__satisfy__se_cmds in Hdenotes'; auto.
+  apply sstate_denotes_state_det with (lc2:=lc2)(gl2:=gl2)(als2:=als2)(Mem2:=Mem2)(tr2:=tr) in Hdenotes'; auto.
+  destruct Hdenotes' as [EQ1 [EQ2 [EQ3 EQ4]]]; subst.
+  eapply dbCmds_eqEnv; eauto.
+Qed.
+
+(* Correctness of the cmds validator *)
+
+Definition tv_cmds (cs1 cs2 : list cmd) (lc gl:GVMap) :=
+se_cmds (mkSstate (env_to_smap gl lc) smem_init sframe_init nil) cs1 =
+se_cmds (mkSstate (env_to_smap gl lc) smem_init sframe_init nil) cs2.
+
+Lemma tv_cmds__is__correct : forall S TD Ps F B cs cs' call0 sbs tmn lc1 arg als1 ECs gl1 Mem1 lc2 als2 gl2 Mem2 tr,
+  uniq gl1 ->
+  uniq lc1 ->  
+  tv_cmds cs cs' lc1 gl1 ->
+  dbCmds (mkState S TD Ps ((mkEC F B ((subblock_intro cs call0)::sbs) tmn lc1 arg als1)::ECs) gl1 Mem1)
+        (mkState S TD Ps ((mkEC F B ((subblock_intro nil call0)::sbs) tmn lc2 arg als2)::ECs) gl2 Mem2)
+        tr ->
+  dbCmds (mkState S TD Ps ((mkEC F B ((subblock_intro cs' call0)::sbs) tmn lc1 arg als1)::ECs) gl1 Mem1)
+        (mkState S TD Ps ((mkEC F B ((subblock_intro nil call0)::sbs) tmn lc2 arg als2)::ECs) gl2 Mem2)
+        tr.
+Proof.
+  intros S TD Ps F B cs cs' call0 sbs tmn lc1 arg0 als1 ECs gl1 Mem1 lc2 als2 gl2 Mem2 tr Huniqg Huniqc Htv_cmds HdbCmds.
+  unfold tv_cmds in Htv_cmds.
+  assert (Uniqs:=HdbCmds).
+  apply dbCmds_uniq in Uniqs; auto.
+  destruct Uniqs as [Uniqg2 Uniqc2].
+  apply op_cmds__satisfy__se_cmds in HdbCmds; auto.
+  rewrite Htv_cmds in HdbCmds.
+  apply se_cmds__denote__op_cmds; auto.
+Qed.
+
+Definition tv_subblock (b1 b2:subblock) (lc gl:GVMap) :=
+match (b1, b2) with
+| (subblock_intro cs1 call1, subblock_intro cs2 call2) =>
+  match (call1, call2) with
+  | (insn_call id1 _ _ _ _ _, insn_call id2 _ _ _ _ _) => 
+    if id1==id2 
+    then
+      let st1 := se_cmds (mkSstate (env_to_smap gl lc) smem_init sframe_init nil) cs1 in
+      let st2 := se_cmds (mkSstate (env_to_smap gl lc) smem_init sframe_init nil) cs2 in
+      let cl1 := se_call st1 call1 in
+      let cl2 := se_call st2 call2 in
+      st1 = st2 /\ cl1 = cl2
+    else
+      False
+  end
+end.
+
+(* Definions below have not been used yet. *)
+
+Fixpoint subst_tt (id0:id) (s0:sterm) (s:sterm) : sterm :=
+match s with
+| sterm_val (value_id id1) => if id0 == id1 then s0 else s
+| sterm_val (value_const c) => sterm_val (value_const c)
+| sterm_bop op sz s1 s2 => 
+    sterm_bop op sz (subst_tt id0 s0 s1) (subst_tt id0 s0 s2)
+| sterm_extractvalue t1 s1 cs => 
+    sterm_extractvalue t1 (subst_tt id0 s0 s1) cs
+| sterm_insertvalue t1 s1 t2 s2 cs => 
+    sterm_insertvalue t1 (subst_tt id0 s0 s1) t2 (subst_tt id0 s0 s2) cs
+| sterm_malloc m1 t1 sz align => 
+    sterm_malloc (subst_tm id0 s0 m1) t1 sz align
+| sterm_alloca m1 t1 sz align => 
+    sterm_alloca (subst_tm id0 s0 m1) t1 sz align
+| sterm_load m1 t1 s1 => 
+    sterm_load (subst_tm id0 s0 m1) t1 (subst_tt id0 s0 s1)
+| sterm_gep inbounds t1 s1 ls2 =>
+    sterm_gep inbounds t1 (subst_tt id0 s0 s1) (List.map (subst_tt id0 s0) ls2)
+| sterm_ext extop t1 s1 t2 => 
+    sterm_ext extop t1 (subst_tt id0 s0 s1) t2
+| sterm_cast castop t1 s1 t2 => 
+    sterm_cast castop t1 (subst_tt id0 s0 s1) t2
+| sterm_icmp cond t1 s1 s2 => 
+    sterm_icmp cond t1 (subst_tt id0 s0 s1) (subst_tt id0 s0 s2)
+| sterm_phi t1 lsl1 => 
+    sterm_phi t1 (List.map 
+                   (fun (sl1:sterm*l) => 
+                    let (s1,l1):=sl1 in 
+                    ((subst_tt id0 s0 s1), l1)
+                   ) 
+                   lsl1)
+| sterm_select s1 t1 s2 s3 => 
+    sterm_select (subst_tt id0 s0 s1) t1 (subst_tt id0 s0 s2) (subst_tt id0 s0 s3)
+end
+with subst_tm (id0:id) (s0:sterm) (m:smem) : smem :=
+match m with 
+| smem_init => smem_init
+| smem_malloc m1 t1 sz align => smem_malloc (subst_tm id0 s0 m1) t1 sz align
+| smem_free m1 t1 s1 => smem_free (subst_tm id0 s0 m1) t1 (subst_tt id0 s0 s1)
+| smem_alloca m1 t1 sz align => smem_alloca (subst_tm id0 s0 m1) t1 sz align
+| smem_load m1 t1 s1 => smem_load (subst_tm id0 s0 m1) t1 (subst_tt id0 s0 s1)
+| smem_store m1 t1 s1 s2 => smem_store (subst_tm id0 s0 m1) t1 (subst_tt id0 s0 s1) (subst_tt id0 s0 s2)
+end
+.
+
+Fixpoint subst_mt (sm:smap) (s:sterm) : sterm :=
+match sm with
+| nil => s
+| (id0, s0)::sm' => subst_mt sm' (subst_tt id0 s0 s)
+end.
+
+Fixpoint subst_mm (sm:smap) (m:smem) : smem :=
+match sm with
+| nil => m
+| (id0, s0)::sm' => subst_mm sm' (subst_tm id0 s0 m)
+end.
+
+
